Full Agent Specification theory, take one

Gvf_Actions.thy
@@ -1,33 +1,39 @@
 (*
-
   Goal verification framework
     - Actions
-  
-  This theory sets up the concepts of agents, actions, transitions and traces.
-  We extend the language for mental state formulas with enabledness of actions.
-  We provide its syntax, semantics and a sound proof system.
-
 *)
+
+\<comment> \<open>This theory sets up the concepts of agents, actions, transitions and traces.
+    We extend the language for mental state formulas with enabledness of actions.
+    We provide its syntax, semantics and a sound proof system.\<close>
+
 theory Gvf_Actions imports Gvf_Mental_States begin
 
 section \<open>Actions\<close>
 
-\<comment> \<open>The identifier for basic actions is a natural number\<close>
+\<comment> \<open>The identifier for basic actions is a natural number.\<close>
 type_synonym Bcap = nat
 
-\<comment> \<open>Agent capability is a basic capability, adopt or drop (the latter two are built into GOAL)\<close>
-datatype cap = basic Bcap | adopt \<Phi>\<^sub>L | drop \<Phi>\<^sub>L
+\<comment> \<open>Agent capability is a basic capability, adopt or drop (the latter two are built into GOAL).\<close>
+datatype cap = basic Bcap | adopt (cget: \<Phi>\<^sub>L) | drop (cget: \<Phi>\<^sub>L)
 
-\<comment> \<open>Type for conditional action that also have a condition on the mental state\<close>
+\<comment> \<open>Auxiliary function.\<close>
+fun is_drop :: \<open>cap \<Rightarrow> bool\<close> where
+  \<open>is_drop (drop _) = True\<close> |
+  \<open>is_drop _ = False\<close>
+
+\<comment> \<open>Type for conditional action that is a pair: a condition on the mental state and a basic action.\<close>
 type_synonym cond_act = \<open>\<Phi>\<^sub>M \<times> cap\<close>
 
-\<comment> \<open>Atoms are extended with enabled for basic/conditional actions\<close>
+\<comment> \<open>Atoms are extended with enabled for basic/conditional actions.\<close>
 datatype Atoms\<^sub>E = Bl \<Phi>\<^sub>L | Gl \<Phi>\<^sub>L | enabled_basic cap | enabled_cond cond_act
+\<comment> \<open>The simple type theory makes it less delicate to extend types, so we redefine the belief
+    and goal operators while adding two new options: one for basic and one for conditional actions.\<close>
 
-\<comment> \<open>The type for mental state formulas concerning enabledness\<close>
+\<comment> \<open>The type for mental state formulas concerning enabledness.\<close>
 type_synonym \<Phi>\<^sub>E = \<open>Atoms\<^sub>E \<Phi>\<^sub>P\<close>
 
-\<comment> \<open>Introduction some notation\<close>
+\<comment> \<open>Introducing some notation.\<close>
 syntax
   "_G" :: \<open>\<Phi>\<^sub>L \<Rightarrow> \<Phi>\<^sub>E\<close> (\<open>G _\<close> 55)
   "_B" :: \<open>\<Phi>\<^sub>L \<Rightarrow> \<Phi>\<^sub>E\<close> (\<open>B _\<close> 55)
@@ -41,76 +47,116 @@ translations
 
 section \<open>Semantics of GOAL\<close>
 
-\<comment> \<open>The type for the function \<T> that gives the agent's belief update capabilities.
-    We replace notion of undefined (from paper) with optional value\<close>
-type_synonym bel_upd_t = \<open>Bcap \<Rightarrow> \<Phi>\<^sub>L set \<Rightarrow> \<Phi>\<^sub>L set option\<close>
+\<comment> \<open>The type for the function \<T> that gives the agent's belief update capabilities.\<close>
+type_synonym bel_upd_t = \<open>Bcap \<Rightarrow> mental_state \<Rightarrow> \<Phi>\<^sub>L set option\<close>
+\<comment> \<open>We replace notion of undefined (from paper) with an optional value, i.e. \<T> a \<Sigma> = None means
+    that basic action a is not defined for \<Sigma>.
+    We further assume that the goal base (entire mental state) is added to the input.\<close>
+
+\<comment> \<open>The mental state transformer gives the agent's mental state update capabilities.\<close>
+fun mental_state_transformer :: \<open>bel_upd_t \<Rightarrow> cap \<Rightarrow> mental_state \<Rightarrow> mental_state option\<close> (\<open>\<M>*\<close>) where
+  \<comment> \<open>If \<T> a \<Sigma> is defined, update the goal base accordingly.\<close>
+  \<open>\<M>* \<T> (basic n) (\<Sigma>, \<Gamma>) = (case \<T> n (\<Sigma>, \<Gamma>) of Some \<Sigma>' \<Rightarrow> Some (\<Sigma>', \<Gamma> - {\<psi> \<in> \<Gamma>. \<Sigma>' \<Turnstile>\<^sub>L \<psi>}) | _ \<Rightarrow> None)\<close> |
+  \<comment> \<open>Remove the goals that entail \<Phi>.\<close>
+  \<open>\<M>* \<T> (drop \<Phi>) (\<Sigma>, \<Gamma>) = Some (\<Sigma>, \<Gamma> - {\<psi> \<in> \<Gamma>. {\<psi>} \<Turnstile>\<^sub>L \<Phi>})\<close> |
+  \<comment> \<open>Add the goal \<Phi> if it is consistent and not entailed by the belief base.\<close>
+  \<open>\<M>* \<T> (adopt \<Phi>) (\<Sigma>, \<Gamma>) = (if \<not> {} \<Turnstile>\<^sub>L \<^bold>\<not> \<Phi> \<and> \<not> \<Sigma> \<Turnstile>\<^sub>L \<Phi> then Some (\<Sigma>, \<Gamma> \<union> {\<Phi>}) else None)\<close>
 
 \<comment> \<open>We fix to a single agent and assume a given belief update function, 
-    a set of conditional actions and an initial state\<close>
+    a set of conditional actions and an initial state.\<close>
 locale single_agent = 
   fixes
     \<T>  :: bel_upd_t and
     \<Pi> :: \<open>cond_act set\<close> and
     M\<^sub>0 :: mental_state
   assumes
-    \<comment> \<open>Non-empty set of conditional actions and initial state is a mental state\<close>
+    \<comment> \<open>Non-empty set of conditional actions and initial state is a mental state.\<close>
     is_agent: \<open>\<Pi> \<noteq> {} \<and> \<nabla> M\<^sub>0\<close> and
-    \<comment> \<open>\<T> preserves consistency\<close>
-    \<T>_consistent: \<open>\<forall>\<Sigma> a. \<Sigma> \<not>\<Turnstile>\<^sub>L \<bottom>\<^sub>L \<longrightarrow> \<T> a \<Sigma> \<noteq> None \<longrightarrow> the (\<T> a \<Sigma>) \<not>\<Turnstile>\<^sub>L \<bottom>\<^sub>L\<close> and
-    \<comment> \<open>\<T> only for defined actions\<close>
-    \<T>_in_domain: \<open>\<T> a \<Sigma> \<noteq> None \<longrightarrow> (\<exists>\<phi>. (\<phi>, basic a) \<in> \<Pi>)\<close>
+    \<comment> \<open>\<T> preserves consistency.\<close>
+    \<T>_consistent: \<open>(\<exists>\<phi>. (\<phi>, basic a) \<in> \<Pi>) \<longrightarrow> \<not> \<Sigma> \<Turnstile>\<^sub>L \<bottom>\<^sub>L \<longrightarrow> \<T> a (\<Sigma>, \<Gamma>) \<noteq> None \<longrightarrow> \<not> the (\<T> a (\<Sigma>, \<Gamma>)) \<Turnstile>\<^sub>L \<bottom>\<^sub>L\<close> and
+    \<comment> \<open>\<T> only for defined actions.\<close>
+    \<T>_in_domain: \<open>\<T> a (\<Sigma>, \<Gamma>) \<noteq> None \<longrightarrow> (\<exists>\<phi>. (\<phi>, basic a) \<in> \<Pi>)\<close>
 
+\<comment> \<open>Working in the context of single_agent, means that we can base definitions, proofs etc. around
+    fixed variables for which a number of assumptions apply. For a specific agent, we need to prove
+    that the assumptions apply for the given input variables. By doing so, we get immediate access
+    to everything defined within the single_agent context.\<close>
 context single_agent
 begin
 
-\<comment> \<open>Basic capabilities derived from the set of conditional actions\<close>
+\<comment> \<open>Basic capabilities derived from the set of conditional actions.\<close>
 definition Cap :: \<open>Bcap set\<close> where
   \<open>Cap \<equiv> { a. \<exists>\<phi>. (\<phi>, (basic a)) \<in> \<Pi> }\<close>
+\<comment> \<open>We assume that a basic capability is represented by at least one conditional action.\<close>
 
-\<comment> \<open>The mental state transformer gives the agent's mental state update capabilities.\<close>
-fun mental_state_transformer :: \<open>cap \<Rightarrow> mental_state \<Rightarrow> mental_state option\<close> (\<open>\<M>\<close>) where
-  \<open>\<M> (basic a) (\<Sigma>, \<Gamma>) = (case \<T> a \<Sigma> of Some \<Sigma>' \<Rightarrow> Some (\<Sigma>', \<Gamma> - {\<psi> \<in> \<Gamma>. \<Sigma>' \<Turnstile>\<^sub>L \<psi>}) | _ => None)\<close> |
-  \<open>\<M> (drop \<Phi>) (\<Sigma>, \<Gamma>) = Some (\<Sigma>, \<Gamma> - {\<psi> \<in> \<Gamma>. {\<psi>} \<Turnstile>\<^sub>L \<Phi>})\<close> |
-  \<open>\<M> (adopt \<Phi>) (\<Sigma>, \<Gamma>) = (if {} \<not>\<Turnstile>\<^sub>L \<^bold>\<not> \<Phi> \<and> \<Sigma> \<not>\<Turnstile>\<^sub>L \<Phi> then Some (\<Sigma>, \<Gamma> \<union> {\<Phi>}) else None)\<close>
+\<comment> \<open>Define mental state transformer local to the agent.\<close>
+abbreviation \<open>\<M> a M \<equiv> \<M>* \<T> a M\<close>
 
-\<comment> \<open>The mental state transformer is only defined for actions of \<Pi>\<close>
-lemma \<M>_some_in_\<Pi>: 
-  assumes \<open>\<M> (basic a) M \<noteq> None\<close> 
-    shows \<open>\<exists>\<phi>. (\<phi>, basic a) \<in> \<Pi>\<close>
-proof (cases M)
-  case (Pair \<Sigma> \<Gamma>)
-  with assms have \<open>\<T> a \<Sigma> \<noteq> None\<close>
-    by (metis (mono_tags, lifting) mental_state_transformer.simps(1) option.case_eq_if)
-  with \<T>_in_domain show ?thesis by simp 
+\<comment> \<open>Examples.\<close>
+lemma 
+  assumes \<open>\<T> n ({P}, {Q}) = Some {P, Q}\<close>
+  shows \<open>\<M> (basic n) ({P}, {Q}) = Some ({P, Q}, {})\<close>
+using assms by simp
+ 
+lemma \<open>\<M> (drop \<top>\<^sub>L) ({}, {P, Q}) = Some ({}, {})\<close> by simp
+
+lemma
+  assumes \<open>\<not> {} \<Turnstile>\<^sub>L \<^bold>\<not> Q\<close> and \<open>\<not> {} \<Turnstile>\<^sub>L Q\<close>
+  shows \<open>\<M> (adopt Q) ({}, {P}) = Some ({}, {P, Q})\<close> 
+proof -
+  have \<open>\<M> (adopt Q) ({}, {P}) = Some ({}, {P} \<union> {Q})\<close> using assms by simp
+  then show ?thesis by auto
 qed
 
-\<comment> \<open>The mental state transformer is only defined for basic capabilities of Cap\<close>
+\<comment> \<open>The mental state transformer is only defined for actions of \<Pi>.\<close>
+lemma \<M>_some_in_\<Pi>: 
+  assumes \<open>\<M> (basic n) M \<noteq> None\<close> 
+    shows \<open>\<exists>\<phi>. (\<phi>, basic n) \<in> \<Pi>\<close>
+proof (cases M)
+  case (Pair \<Sigma> \<Gamma>)
+  with assms obtain \<Sigma>' \<Gamma>' where someM: \<open>\<M> (basic n) (\<Sigma>, \<Gamma>) = Some (\<Sigma>', \<Gamma>')\<close> by auto
+  then have \<open>\<T> n (\<Sigma>, \<Gamma>) = Some \<Sigma>'\<close>
+  proof (cases \<open>\<T> n (\<Sigma>, \<Gamma>)\<close>)
+    case None
+    then have \<open>\<M> (basic n) (\<Sigma>, \<Gamma>) = None\<close> by simp
+    with someM show ?thesis by simp
+  next
+    case (Some \<Sigma>'')
+    moreover have \<open>fst (the (\<M> (basic n) (\<Sigma>, \<Gamma>))) = \<Sigma>''\<close> using Some by simp
+    moreover have \<open>fst (the (\<M> (basic n) (\<Sigma>, \<Gamma>))) = \<Sigma>'\<close> using someM by simp
+    ultimately show ?thesis by simp
+  qed    
+  with \<T>_in_domain show ?thesis by blast
+qed
+
+\<comment> \<open>The mental state transformer is only defined for basic capabilities of Cap.\<close>
 lemma \<M>_some_Cap:
   assumes \<open>\<M> (basic a) M \<noteq> None\<close> 
   shows \<open>a \<in> Cap\<close>
 using assms \<M>_some_in_\<Pi> Cap_def by auto
 
-\<comment> \<open>Mental state transformer preserves mental state constraints when \<T> preserves consistency\<close>
+\<comment> \<open>Mental state transformer preserves properties of mental states (when \<T> preserves consistency).\<close>
 lemma \<M>_preserves_mst: \<open>\<nabla> (\<Sigma>, \<Gamma>) \<Longrightarrow> \<M> c (\<Sigma>, \<Gamma>) \<noteq> None \<Longrightarrow> \<nabla> (the (\<M> c (\<Sigma>, \<Gamma>)))\<close>
 proof (induct c)
   case basic: (basic a)
-  then obtain \<Sigma>' where \<Sigma>': \<open>\<T> a \<Sigma> = Some \<Sigma>'\<close> by fastforce
+  then obtain \<Sigma>' where \<Sigma>': \<open>\<T> a (\<Sigma>, \<Gamma>) = Some \<Sigma>'\<close> by fastforce
   have \<open>\<nabla> (\<Sigma>', \<Gamma> - {\<psi> \<in> \<Gamma>. \<Sigma>' \<Turnstile>\<^sub>L \<psi>})\<close> (is \<open>\<nabla> (\<Sigma>', ?\<Gamma>')\<close>)
   proof -
-    have \<open>\<Sigma>' \<not>\<Turnstile>\<^sub>L \<bottom>\<^sub>L\<close>
+    have \<open>\<not> \<Sigma>' \<Turnstile>\<^sub>L \<bottom>\<^sub>L\<close>
     proof -
-      from basic(1) have \<open>\<Sigma> \<not>\<Turnstile>\<^sub>L \<bottom>\<^sub>L\<close> unfolding is_mental_state_def by simp
-      with basic(2) have \<open>the (\<T> a \<Sigma>) \<not>\<Turnstile>\<^sub>L \<bottom>\<^sub>L\<close> using \<Sigma>' \<T>_consistent by blast
+      from basic(1) have \<open>\<not> \<Sigma> \<Turnstile>\<^sub>L \<bottom>\<^sub>L\<close> unfolding is_mental_state_def by simp
+      moreover have \<open>\<exists>\<phi>. (\<phi>, basic a) \<in> \<Pi>\<close> using \<M>_some_in_\<Pi> basic.prems(2) by blast
+      ultimately have \<open>\<not> the (\<T> a (\<Sigma>, \<Gamma>)) \<Turnstile>\<^sub>L \<bottom>\<^sub>L\<close> using \<Sigma>' \<T>_consistent basic(2) by blast
       with \<Sigma>' show ?thesis by simp
     qed
-    moreover from basic(1) have \<open>\<forall>\<gamma>\<in>?\<Gamma>'. \<Sigma> \<not>\<Turnstile>\<^sub>L \<gamma> \<and> {} \<not>\<Turnstile>\<^sub>L \<^bold>\<not> \<gamma>\<close> 
+    moreover from basic(1) have \<open>\<forall>\<gamma>\<in>?\<Gamma>'. \<not> \<Sigma> \<Turnstile>\<^sub>L \<gamma> \<and> \<not> {} \<Turnstile>\<^sub>L \<^bold>\<not> \<gamma>\<close> 
       unfolding is_mental_state_def by simp
     ultimately show ?thesis unfolding is_mental_state_def by simp
   qed
   with \<Sigma>' show ?case by simp 
 next
   case adopt: (adopt \<Phi>)
-  then have mst_goal: \<open>{} \<not>\<Turnstile>\<^sub>L \<^bold>\<not> \<Phi> \<and> \<Sigma> \<not>\<Turnstile>\<^sub>L \<Phi>\<close> by fastforce
+  with mental_state_transformer.simps(3) have mst_goal: \<open>\<not> {} \<Turnstile>\<^sub>L \<^bold>\<not> \<Phi> \<and> \<not> \<Sigma> \<Turnstile>\<^sub>L \<Phi>\<close> by metis
   with adopt(1) have \<open>\<nabla> (\<Sigma>, \<Gamma> \<union> {\<Phi>})\<close> unfolding is_mental_state_def by simp 
   with mst_goal show ?case by simp
 next
@@ -121,42 +167,64 @@ qed
 
 section \<open>Traces\<close>
 
-\<comment> \<open>Transition relation between states due to an action\<close>
+\<comment> \<open>Transition relation between states due to an action.\<close>
 definition transition :: \<open>mental_state \<Rightarrow> cond_act \<Rightarrow> mental_state \<Rightarrow> bool\<close> (\<open>_ \<rightarrow>_ _\<close>) where
   \<open>M \<rightarrow>b M' \<equiv> let (\<phi>, a) = b in b \<in> \<Pi> \<and> M \<Turnstile>\<^sub>M \<phi> \<and> \<M> a M = Some M'\<close>
+\<comment> \<open>If b is a conditional action, and the condition true in M, then there is possible transition
+    between M and M' where M' is the result of applying \<M> for a to M.\<close>
 
-\<comment> \<open>Chain of transitions (computation steps) gives the computation relation\<close>
+\<comment> \<open>Chain of transitions (computation steps) gives the computation relation.\<close>
 inductive computation :: \<open>mental_state \<Rightarrow> mental_state \<Rightarrow> bool\<close> (\<open>_ \<rightarrow>* _\<close>) where
+  \<comment> \<open>The base step from the initial mental state.\<close>
   basis: \<open>M\<^sub>0 \<rightarrow>b M' \<Longrightarrow> M\<^sub>0 \<rightarrow>* M'\<close> |
+  \<comment> \<open>Inductive step from an existing computation given a transition.\<close>
   step: \<open>M \<rightarrow>* M' \<Longrightarrow> M' \<rightarrow>b M'' \<Longrightarrow> M \<rightarrow>* M''\<close>
 
-\<comment> \<open>Traces are infinite structures\<close>
-codatatype trace = TCons (thd: mental_state) (ttl: \<open>(cond_act \<times> trace)\<close>)
+\<comment> \<open>Example\<close>
+lemma \<open>M\<^sub>0 \<rightarrow>a M\<^sub>1 \<Longrightarrow> M\<^sub>1 \<rightarrow>b M\<^sub>2 \<Longrightarrow> M\<^sub>0 \<rightarrow>* M\<^sub>2\<close>
+  using basis step by blast
 
-\<comment> \<open>Retrieve the nth conditional action of the trace\<close>
+\<comment> \<open>Traces are infinite structures.\<close>
+codatatype trace = Trace mental_state \<open>cond_act \<times> trace\<close>
+\<comment> \<open>trace := mental state, conditional action, trace\<close>
+
+\<comment> \<open>Example.\<close>
+value \<open>Trace M\<^sub>0 (a, (Trace M\<^sub>1 (b, (Trace M\<^sub>2 X))))\<close>
+
+\<comment> \<open>Retrieve the nth conditional action of the trace.\<close>
 fun act_nth :: \<open>trace \<Rightarrow> nat \<Rightarrow> cond_act\<close> where
-  \<open>act_nth (TCons _ (b, _)) 0 = b\<close> |
-  \<open>act_nth (TCons _ (_, S)) n = act_nth S (n-1)\<close>
+  \<open>act_nth (Trace _ (b, _)) 0 = b\<close> |
+  \<open>act_nth (Trace _ (_, S)) n = act_nth S (n-1)\<close>
 
-\<comment> \<open>Retriece the nth mental state of the trace\<close>
+\<comment> \<open>Example.\<close>
+lemma \<open>b = act_nth (Trace M\<^sub>0 (a, (Trace M\<^sub>1 (b, (Trace M\<^sub>2 X))))) 1\<close> by simp
+
+\<comment> \<open>Retrieve the nth mental state of the trace.\<close>
 fun st_nth :: \<open>trace \<Rightarrow> nat \<Rightarrow> mental_state\<close> where
-  \<open>st_nth (TCons M _) 0 = M\<close> |
-  \<open>st_nth (TCons _ (_, S)) n = st_nth S (n-1)\<close>
+  \<open>st_nth (Trace M (_, _)) 0 = M\<close> |
+  \<open>st_nth (Trace _ (_, S)) n = st_nth S (n-1)\<close>
 
-\<comment> \<open>Useful lemmas about equality and fetching of condition/action for a nth conditional action\<close>
+\<comment> \<open>Example.\<close>
+lemma \<open>M\<^sub>1 = st_nth (Trace M\<^sub>0 (a, (Trace M\<^sub>1 (b, (Trace M\<^sub>2 X))))) 1\<close> by simp
+
+\<comment> \<open>if (\<psi>, a) is the ith conditional action of trace s, then the first value of (act_nth s i)
+    is \<psi>. This is intuitively easy to see, but pattern matching using equality can be problematic.\<close>
 lemma fst_act_nth: \<open>(\<psi>, a) = act_nth s i \<Longrightarrow> fst (act_nth s i) = \<psi>\<close>
   by (metis fstI)
 
+\<comment> \<open>The same as above but for the second value.\<close>
 lemma snd_act_nth: \<open>(\<psi>, a) = act_nth s i \<Longrightarrow> snd (act_nth s i) = a\<close>
   by (metis sndI)
 
-\<comment> \<open>The trace definition using the type\<close>
+\<comment> \<open>The definition of a trace (not every element of the datatype trace qualifies).\<close>
 definition is_trace :: \<open>trace \<Rightarrow> bool\<close> where
   \<open>is_trace s \<equiv> 
     \<forall>i. (let (M, M', (\<phi>, a)) = (st_nth s i, st_nth s (i+1), act_nth s i) in 
           (\<phi>, a) \<in> \<Pi> \<and> ((M \<rightarrow>(\<phi>, a) M') \<or> \<M> a M = None \<and> M = M'))\<close>
+\<comment> \<open>For all i there is a transition between M_i and M_(i+1) due to an action, or the action
+    is not enabled and the successor state (M_(i+1)) is equal to the current (M_i).\<close>
 
-\<comment> \<open>The nth conditional action of a trace is in \<Pi>\<close>
+\<comment> \<open>The nth conditional action of a trace is in \<Pi>.\<close>
 lemma trace_in_\<Pi>:
   assumes \<open>is_trace s\<close>
   shows \<open>\<forall>i. (act_nth s i) \<in> \<Pi>\<close>
@@ -170,7 +238,7 @@ proof
   then show \<open>(act_nth s i) \<in> \<Pi>\<close> by simp
 qed
 
-\<comment> \<open>If there is not transition between two neighbouring states in trace, then they are equal\<close>
+\<comment> \<open>If there is no transition between a state and its successor in a trace, they must be equal.\<close>
 lemma not_transition_eq:
   assumes \<open>is_trace s\<close>
   shows \<open>\<not>((st_nth s i) \<rightarrow>(act_nth s i) (st_nth s (i+1))) \<longrightarrow> (st_nth s i) = (st_nth s (i+1))\<close>
@@ -184,18 +252,18 @@ proof
   then show \<open>?M = ?M'\<close> by auto
 qed
 
-\<comment> \<open>A fair trace ensures that there always is a future point where an actions is scheduled\<close>
+\<comment> \<open>A fair trace ensures that there always is a future point where an actions is scheduled.\<close>
 definition fair_trace :: \<open>trace \<Rightarrow> bool\<close> where
   \<open>fair_trace s \<equiv> \<forall> b \<in> \<Pi> . \<forall>i . \<exists> j > i. act_nth s j = b\<close>
 
-\<comment> \<open>Meaning of an agent\<close>
+\<comment> \<open>An agent is defined as the set of fair traces starting from the initial state.\<close>
 definition Agent :: \<open>trace set\<close> where
   \<open>Agent \<equiv> {s . is_trace s \<and> fair_trace s \<and> st_nth s 0 = M\<^sub>0}\<close>
 
-\<comment> \<open>If the mental state transformer is defined for a state in the trace, then it gives the successor state\<close>
+\<comment> \<open>If the mental state transformer is defined for a state in the trace, then it gives the successor state.\<close>
 lemma \<M>_suc_state:
   assumes \<open>s \<in> Agent\<close>
-      and \<open>(\<phi>, a) = (act_nth s i)\<close>
+      and \<open>(\<phi>, a) = act_nth s i\<close>
       and \<open>\<M> a (st_nth s i) \<noteq> None\<close>
     shows \<open>st_nth s (i+1) = the (\<M> a (st_nth s i))\<close>
       (is \<open>?M' = the (\<M> a ?M)\<close>)
@@ -208,9 +276,39 @@ proof -
   then show ?thesis unfolding transition_def by simp
 qed
 
+\<comment> \<open>All states in trace comply to mental state definition.\<close>
+lemma is_mst_trace: 
+  assumes \<open>s \<in> Agent\<close>
+  shows   \<open>\<nabla> (st_nth s n)\<close>
+proof (induct n)
+  case 0
+  with assms show ?case using is_agent unfolding Agent_def by simp
+next
+  case (Suc n)
+  let ?M = \<open>st_nth s n\<close> and ?M' = \<open>st_nth s (Suc n)\<close> and ?b = \<open>act_nth s n\<close>
+  have trace_n: \<open>(?M \<rightarrow>?b ?M') \<or> \<M> (snd ?b) ?M = None \<and> ?M = ?M'\<close>
+  proof -
+    from assms(1) have \<open>is_trace s\<close> unfolding Agent_def by simp
+    then have \<open>let (\<phi>, a) = ?b in (\<phi>, a) \<in> \<Pi> \<and> ((?M \<rightarrow>(\<phi>, a) ?M') \<or> \<M> a ?M = None \<and> ?M = ?M')\<close>
+      unfolding is_trace_def by simp
+    then show ?thesis by auto
+  qed
+  then show ?case 
+  proof (cases \<open>\<M> (snd ?b) ?M = None\<close>)
+    case True
+    with Suc trace_n show ?thesis unfolding transition_def by auto
+  next
+    case False
+    with \<M>_preserves_mst have \<open>\<nabla> (the (\<M> (snd ?b) ?M))\<close> 
+      using Suc by (cases ?M) simp
+    with \<M>_suc_state trace_n show ?thesis using assms False unfolding Agent_def
+      by (metis (no_types, lifting) Suc_eq_plus1 prod.collapse)
+  qed
+qed
+
 section \<open>Derivability\<close>
 
-\<comment> \<open>Auxiliary function that converts mental state formulas to the type including enabledness\<close>
+\<comment> \<open>Auxiliary function that converts mental state formulas to the type including enabledness.\<close>
 fun to_\<Phi>\<^sub>E :: \<open>\<Phi>\<^sub>M \<Rightarrow> \<Phi>\<^sub>E\<close> (\<open>_\<^sup>E\<close>) where
   \<open>(Atom (Atoms\<^sub>M.Bl \<Phi>))\<^sup>E = Atom (Bl \<Phi>)\<close> |
   \<open>(Atom (Atoms\<^sub>M.Gl \<Phi>))\<^sup>E = Atom (Gl \<Phi>)\<close> |
@@ -219,32 +317,43 @@ fun to_\<Phi>\<^sub>E :: \<open>\<Phi>\<^sub>M \<Rightarrow> \<Phi>\<^sub>E\<clo
   \<open>(\<phi>\<^sub>1 \<^bold>\<or> \<phi>\<^sub>2)\<^sup>E = (\<phi>\<^sub>1\<^sup>E) \<^bold>\<or> (\<phi>\<^sub>2\<^sup>E)\<close> |
   \<open>(\<phi>\<^sub>1 \<^bold>\<and> \<phi>\<^sub>2)\<^sup>E = (\<phi>\<^sub>1\<^sup>E) \<^bold>\<and> (\<phi>\<^sub>2\<^sup>E)\<close>
 
-\<comment> \<open>Truth of enabledness (semantics)\<close>
+\<comment> \<open>Truth of enabledness (semantics).\<close>
 fun semantics\<^sub>E' :: \<open>mental_state \<Rightarrow> Atoms\<^sub>E \<Rightarrow> bool\<close> where
+  \<comment> \<open>Semantics of B and G are the same as for mental state formulas without enabled.\<close>
   \<open>semantics\<^sub>E' M (Bl \<Phi>) = semantics\<^sub>M' M (Atoms\<^sub>M.Bl \<Phi>)\<close> |
   \<open>semantics\<^sub>E' M (Gl \<Phi>) = semantics\<^sub>M' M (Atoms\<^sub>M.Gl \<Phi>)\<close> |
-  \<open>semantics\<^sub>E' M (enabled_basic (basic a)) = (a \<in> Cap \<and> \<M> (basic a) M \<noteq> None)\<close> |
-  \<open>semantics\<^sub>E' M (enabled_basic (adopt \<Phi>)) = (\<M> (adopt \<Phi>) M \<noteq> None)\<close> |
-  \<open>semantics\<^sub>E' M (enabled_basic (drop \<Phi>)) = (\<M> (drop \<Phi>) M \<noteq> None)\<close> |
+  \<comment> \<open>a is defined for the action and \<M> a is defined for  M.\<close>
+  \<open>semantics\<^sub>E' M (enabled_basic a) = (\<M> a M \<noteq> None)\<close> |
+  \<comment> \<open>Conditional action b is enabled if there exists a transition from M to M' using b for some M'.\<close>
   \<open>semantics\<^sub>E' M (enabled_cond b) = (\<exists>M'. (M \<rightarrow>b M'))\<close>
 
+\<comment> \<open>Semantics of atoms with enabled can be seen as an interpretation given a mental state.\<close>
 abbreviation semantics\<^sub>E :: \<open>mental_state \<Rightarrow> \<Phi>\<^sub>E \<Rightarrow> bool\<close> (infix \<open>\<Turnstile>\<^sub>E\<close> 50) where
   \<open>M \<Turnstile>\<^sub>E \<phi> \<equiv> semantics\<^sub>P (semantics\<^sub>E' M) \<phi>\<close>
 
-\<comment> \<open>Proof system\<close>
+\<comment> \<open>Example.\<close>
+lemma \<open>(M\<^sub>0 \<rightarrow>b M\<^sub>1) \<Longrightarrow> M\<^sub>0 \<Turnstile>\<^sub>E enabled b\<close> 
+proof -
+  assume \<open>M\<^sub>0 \<rightarrow>b M\<^sub>1\<close>
+  then have \<open>\<exists>M'. (M\<^sub>0 \<rightarrow>b M')\<close> by blast
+  then show \<open>M\<^sub>0 \<Turnstile>\<^sub>E enabled b\<close> by simp
+qed
+
+\<comment> \<open>Proof system.\<close>
 inductive provable\<^sub>E :: \<open>\<Phi>\<^sub>E \<Rightarrow> bool\<close> (\<open>\<turnstile>\<^sub>E _\<close> 40) where
-  \<comment> \<open>Derive classical tautologies\<close>
+  \<comment> \<open>Derive classical tautologies.\<close>
   R1: \<open>\<turnstile>\<^sub>P \<phi> \<Longrightarrow> \<turnstile>\<^sub>E \<phi>\<close> |
-  \<comment> \<open>Properties of beliefs and goal s\<close>
+  \<comment> \<open>Properties of beliefs and goals. Imported from proof system for mental state formulas.\<close>
   R\<^sub>M: \<open>\<turnstile>\<^sub>M \<phi> \<Longrightarrow> \<turnstile>\<^sub>E (\<phi>\<^sup>E)\<close> |
-  \<comment> \<open>Enabledness\<close>
+  \<comment> \<open>Properties of enabled.\<close>
   E1: \<open>\<turnstile>\<^sub>P \<phi> \<Longrightarrow> \<turnstile>\<^sub>E (enabledb a) \<Longrightarrow> (\<phi> \<triangleright> do a) \<in> \<Pi> \<Longrightarrow> \<turnstile>\<^sub>E (enabled (\<phi> \<triangleright> do a))\<close> |
   E2: \<open>\<turnstile>\<^sub>E (enabledb (drop \<Phi>))\<close> |
   R3: \<open>\<not> \<turnstile>\<^sub>P \<^bold>\<not> \<Phi> \<Longrightarrow> \<turnstile>\<^sub>E (\<^bold>\<not> ((B \<Phi>)\<^sup>E) \<^bold>\<longleftrightarrow> (enabledb (adopt \<Phi>)))\<close> |
   R4: \<open>\<turnstile>\<^sub>P (\<^bold>\<not> \<Phi>) \<Longrightarrow> \<turnstile>\<^sub>E (\<^bold>\<not> (enabledb (adopt \<Phi>)))\<close> |
-  R5: \<open>\<forall>\<Sigma>. \<T> a \<Sigma> \<noteq> None \<Longrightarrow> \<turnstile>\<^sub>E (enabledb (basic a))\<close>
+  R5: \<open>\<forall>M. \<T> a M \<noteq> None \<Longrightarrow> \<turnstile>\<^sub>E (enabledb (basic a))\<close>
 
-\<comment> \<open>Soundness\<close>
+section \<open>Soundness\<close>
+
 lemma soundness\<^sub>E:
   assumes \<open>\<nabla> M\<close>
   shows \<open>\<turnstile>\<^sub>E \<phi> \<Longrightarrow> M \<Turnstile>\<^sub>E \<phi>\<close>
@@ -266,7 +375,7 @@ next
   then show ?case 
   proof (cases a)
     case (basic n)
-    with E1.hyps(3) obtain M' where \<open>n \<in> Cap \<and> \<M> a M = Some M'\<close> by auto
+    with E1.hyps(3) obtain M' where \<open>\<M> a M = Some M'\<close> by auto
     with \<open>M \<Turnstile>\<^sub>M \<phi>\<close> have \<open>M \<rightarrow>(\<phi> \<triangleright> do a) M'\<close> using E1(4) 
       unfolding transition_def by simp
     then have \<open>\<exists>M'. (M \<rightarrow>(\<phi> \<triangleright> do a) M')\<close> by blast
@@ -306,8 +415,8 @@ next
     show \<open>\<forall>\<Gamma>. (\<Sigma>, \<Gamma>) \<Turnstile>\<^sub>E Atom (enabled_basic (basic a))\<close>
     proof
       fix \<Gamma>
-      from \<open>\<forall>\<Sigma>. \<T> a \<Sigma> \<noteq> None\<close> have \<open>\<T> a \<Sigma> \<noteq> None\<close> \<open>a \<in> Cap\<close> using \<T>_in_domain unfolding Cap_def 
-        by simp_all
+      from \<open>\<forall>M. \<T> a M \<noteq> None\<close> have \<open>\<T> a (\<Sigma>, \<Gamma>) \<noteq> None\<close> \<open>a \<in> Cap\<close> 
+        using \<T>_in_domain unfolding Cap_def by simp_all
       then show \<open>(\<Sigma>, \<Gamma>) \<Turnstile>\<^sub>E Atom (enabled_basic (basic a))\<close> by auto
     qed
   qed
@@ -315,7 +424,7 @@ next
   then show ?case by blast
 qed
 
-\<comment> \<open>The semantics of a converted formula is equal to the original\<close>
+\<comment> \<open>The semantics of a converted formula is equal to the original.\<close>
 lemma transfer_semantics\<^sub>M: \<open>M \<Turnstile>\<^sub>M \<phi> \<longleftrightarrow> M \<Turnstile>\<^sub>E (\<phi>\<^sup>E)\<close> 
 proof (induct \<phi>)
   case (Atom x)
