Gvf_Agent_Specification.thy
@@ -1,60 +1,341 @@
 (*
-
   Goal verification framework
-    - Agent Specification
-  
-  This theory sets up the framework for specifying agents by means of predicates for enabledness 
-  and Hoare triple axioms  instead of providing a function for \<T>. Instead, adopt the idea that 
-  we may assume the agent specification reflects the actual model, i.e. the \<T> function complies 
-  to our specification.
-
-  TODO: Proof system and more
-
+    - Agent Specification  
 *)
+\<comment> \<open>This theory sets up the framework for specifying agents by means of predicates for enabledness 
+    and Hoare triple axioms  instead of providing a function for \<T>. Instead, adopt the idea that 
+    we may assume the agent specification reflects the actual model, i.e. the \<T> function complies 
+    to our specification.\<close>
+
 theory Gvf_Agent_Specification imports Gvf_Hoare_Logic begin
 
-\<comment> \<open>A type for the specification of enabledness and Hoare triple axioms\<close>
-type_synonym ht_specification = \<open>(\<Phi>\<^sub>M \<times> hoare_triple) set\<close>
+\<comment> \<open>A type for the specification of enabledness and Hoare triple axioms.\<close>
+type_synonym ht_specification = \<open>(Bcap \<times> \<Phi>\<^sub>M \<times> hoare_triple list) list\<close>
+\<comment> \<open>Set of pairs of mental state formula (enabled) and set of Hoare triple axioms.\<close>
+
+section \<open>Satisfiability of specification\<close>
+
+\<comment> \<open>The main idea behind this, and the following, section is that we now base agents on specifications.
+    We do not want to state the belief update function for an agent specifically. As such, we need
+    a link between agent specification and belief update function. We can reduce this problem to the
+    problem of proving the existence of a belief update function (model) given a specification.\<close>
+
+\<comment> \<open>Satisfiability of a specification.\<close>
+definition satisfiable :: \<open>ht_specification \<Rightarrow> bool\<close> where
+  \<open>satisfiable S \<equiv> 
+    \<comment> \<open>Quantify over all mental states. Go through each element s in S.\<close>
+    \<forall>M. \<forall>s \<in> set S. 
+      \<comment> \<open>Get fields in s. Define a variable for the set of preconditions satisfied by M.\<close>
+      (let (_, \<Phi>, hts) = s; sat_hts = { ht \<in> set hts. M \<Turnstile>\<^sub>M pre ht } in
+        \<comment> \<open>If the basic action is enabled (\<Phi>)\<close>
+        (M \<Turnstile>\<^sub>M \<Phi> \<longrightarrow> 
+          \<comment> \<open>There exists a mental state M'...\<close>
+          (\<exists>M'. 
+            \<comment> \<open>That preserves consistency, and ...\<close>
+            (\<not> fst M \<Turnstile>\<^sub>L \<bottom>\<^sub>L \<longrightarrow> \<not> fst M' \<Turnstile>\<^sub>L \<bottom>\<^sub>L) \<and> 
+            \<comment> \<open>Where the goal base is obtained by removing achieved goals, and ...\<close>
+            (snd M' = snd M - {\<psi> \<in> snd M. fst M' \<Turnstile>\<^sub>L \<psi>}) \<and> 
+            \<comment> \<open>That satisfy all of the Hoare triples for this basic action.\<close>
+            (\<forall>ht \<in> sat_hts. M' \<Turnstile>\<^sub>M post ht))) \<and>
+        \<comment> \<open>If the basic action is not enabled, the Hoare triples should be satisfied by M.\<close>
+        (M \<Turnstile>\<^sub>M \<^bold>\<not> \<Phi> \<longrightarrow> (\<forall>ht \<in> sat_hts. M \<Turnstile>\<^sub>M post ht)))\<close>
+
+
+\<comment> \<open>We restrict those elements of the type 'ht_specification' that are valid specifications.\<close>
+\<comment> \<open>Hoare triples only for basic actions and should be for grouped for actions.\<close>
+fun is_ht_specification_hts :: \<open>Bcap \<Rightarrow> hoare_triple list \<Rightarrow> bool\<close>  where
+  \<open>is_ht_specification_hts n hts = 
+    (\<forall>ht\<in> set hts. is_htb_basic ht \<and> fst (snd (the (htb_basic_unpack ht))) = n)\<close>
+
+\<comment> \<open>Main definition. Each action (group) can only appear once, S is satisfiable and each element
+   s of S satisfy the function defined above.\<close>
+definition is_ht_specification :: \<open>ht_specification \<Rightarrow> bool\<close> where
+  \<open>is_ht_specification S \<equiv> distinct (map fst S) \<and> satisfiable S \<and> 
+                            (\<forall>s \<in> set S. is_ht_specification_hts (fst s) (snd (snd s)))\<close>
 
 \<comment> \<open>State that a given \<T> complies to our assumptions, partly due to semantics of Hoare triples
     and partly due to the properties about the fixed agent\<close>
-definition complies :: \<open>cond_act set \<Rightarrow> ht_specification \<Rightarrow> bel_upd_t \<Rightarrow> bool\<close> where
-  \<open>complies \<Pi> S \<T> \<equiv>
-    (\<forall>\<Sigma> a. \<Sigma> \<not>\<Turnstile>\<^sub>L \<bottom>\<^sub>L \<longrightarrow> \<T> a \<Sigma> \<noteq> None \<longrightarrow> the (\<T> a \<Sigma>) \<not>\<Turnstile>\<^sub>L \<bottom>\<^sub>L) \<and>
-    (\<forall>\<Sigma> a. \<T> a \<Sigma> \<noteq> None \<longrightarrow> (\<exists>\<phi>'. (\<phi>', basic a) \<in> \<Pi>)) \<and> 
-    (\<forall>(\<Phi>, ht)\<in>S. 
-      (case ht of htb \<phi> (basic n) \<psi> \<Rightarrow>
-        (\<forall>M. M \<Turnstile>\<^sub>M \<Phi> \<^bold>\<and> \<phi> \<longrightarrow> (the (\<T> n (fst M)), snd M) \<Turnstile>\<^sub>M \<psi> \<and> M \<Turnstile>\<^sub>M \<^bold>\<not>\<Phi> \<^bold>\<and> \<phi> \<longrightarrow> M \<Turnstile>\<^sub>M \<psi>)))\<close>
+fun complies_ht :: \<open>mental_state \<Rightarrow> bel_upd_t \<Rightarrow> \<Phi>\<^sub>M \<Rightarrow> (\<Phi>\<^sub>M \<times> Bcap \<times> \<Phi>\<^sub>M) \<Rightarrow> bool\<close> where
+  \<open>complies_ht M \<T> \<Phi> (\<phi>, n, \<psi>) =
+    \<comment> \<open>\<Phi> specify if the action is enabled\<close>
+    ((M \<Turnstile>\<^sub>M \<Phi> \<longleftrightarrow> \<T> n M \<noteq> None) \<and>
+    \<comment> \<open>Transitions preserves consistency.\<close>
+    (\<not> (fst M) \<Turnstile>\<^sub>L \<bottom>\<^sub>L \<longrightarrow> \<T> n M \<noteq> None \<longrightarrow> \<not>the (\<T> n M) \<Turnstile>\<^sub>L \<bottom>\<^sub>L) \<and>
+    \<comment> \<open>Basic Hoare triple semantics for action enabled.\<close>
+    (M \<Turnstile>\<^sub>M \<phi> \<and> M \<Turnstile>\<^sub>M \<Phi> \<longrightarrow> the (\<M>* \<T> (basic n) M) \<Turnstile>\<^sub>M \<psi>) \<and>
+    \<comment> \<open>Basic Hoare triple semantics for action not enabled.\<close>
+    (M \<Turnstile>\<^sub>M \<phi> \<and> M \<Turnstile>\<^sub>M \<^bold>\<not> \<Phi> \<longrightarrow> M \<Turnstile>\<^sub>M \<psi>))\<close>
+
+\<comment> \<open>Does an element s of S comply to a given belief update function?\<close>
+definition complies_hts :: \<open>(Bcap \<times> \<Phi>\<^sub>M \<times> hoare_triple list) \<Rightarrow> bel_upd_t \<Rightarrow> bool\<close> where
+  \<open>complies_hts s \<T> \<equiv>
+    \<comment> \<open>For all Hoare triples for this action...\<close>
+    \<forall>ht\<in>set (snd (snd s)). 
+      \<comment> \<open>It is for basic actions, and ...\<close>  
+      is_htb_basic ht \<and> 
+      \<comment> \<open>It complies for all mental states.\<close>
+      (\<forall>M. complies_ht M \<T> (fst (snd s)) (the (htb_basic_unpack ht)))\<close>
+
+\<comment> \<open>Main definition. Does the specification comply to a given belief update function?\<close>
+definition complies :: \<open>ht_specification \<Rightarrow> bel_upd_t \<Rightarrow> bool\<close> where
+  \<open>complies S \<T> \<equiv> (\<forall>s\<in>set S. complies_hts s \<T> \<and> (\<forall>n. n \<notin> set (map fst S) \<longrightarrow> (\<forall>M. \<T> n M = None)))\<close>
+
+section \<open>Model existence\<close>
+
+\<comment> \<open>Showing existence of a model that complies can be done separately for each group of Hoare triples.\<close>
+lemma model_exists_disjoint: 
+  assumes \<open>is_ht_specification S\<close>
+     and  \<open>\<forall>s\<in>set S. \<exists>\<T>. complies_hts s \<T>\<close>
+    shows \<open>\<exists>\<T>. complies S \<T>\<close>
+proof 
+  from assms(1) have \<open>distinct (map fst S)\<close> unfolding is_ht_specification_def by simp
+  let ?\<T> = \<open>\<lambda>n. if n \<in> set (map fst S) then (SOME \<T>. complies_hts (THE s'. s'\<in>set S \<and> n = fst s') \<T>) n else (\<lambda>M. None)\<close>
+  show \<open>complies S ?\<T>\<close> unfolding complies_def 
+  proof
+    fix s   
+    assume member: \<open>s \<in> set S\<close>
+    have \<open>complies_hts s ?\<T>\<close>    
+    proof (cases s)
+      case f1: (fields n \<Phi> hts)
+      have \<open>\<forall>ht\<in>set hts. \<forall>M. complies_ht M ?\<T> \<Phi> (the (htb_basic_unpack ht))\<close>
+      proof
+        fix ht
+        assume \<open>ht \<in> set hts\<close>
+        show \<open>\<forall>M. complies_ht M ?\<T> \<Phi> (the (htb_basic_unpack ht))\<close>
+        proof
+          fix M
+          show \<open>complies_ht M ?\<T> \<Phi> (the (htb_basic_unpack ht))\<close>
+          proof (cases \<open>(the (htb_basic_unpack ht))\<close>)
+            case (fields \<phi> n' \<psi>)
+            have \<open>s\<in>set S \<and> fst s = fst s\<close> using \<open>s \<in> set S\<close> by simp
+            moreover have \<open>\<forall>s'. s'\<in>set S \<and> fst s = fst s' \<longrightarrow> s' = s\<close> using \<open>distinct (map fst S)\<close>
+              by (metis member eq_key_imp_eq_value prod.collapse)
+            ultimately have \<open>(THE s'. s'\<in>set S \<and> fst s = fst s') = s\<close> using the_equality by auto
+            then have \<open>?\<T> (fst s) = (SOME \<T>. complies_hts s \<T>) (fst s)\<close> (is \<open>?\<T> (fst s) = ?\<T>' (fst s)\<close>) using member by simp
+            have \<open>\<exists>\<T>. complies_hts s \<T>\<close> using assms(2) member by simp
+            then have \<open>complies_hts s ?\<T>'\<close> using someI_ex[where ?P=\<open>complies_hts s\<close>] by simp
+            then have \<open>\<forall>ht\<in>set hts. is_htb_basic ht \<and> (\<forall>M. complies_ht M ?\<T>' \<Phi> (the (htb_basic_unpack ht)))\<close> 
+              using f1 complies_hts_def by fastforce
+            with f1 \<open>ht \<in> set hts\<close> have \<open>\<forall>M. complies_ht M ?\<T>' \<Phi> (the (htb_basic_unpack ht))\<close> by simp
+            then have \<open>complies_ht M ?\<T>' \<Phi> (the (htb_basic_unpack ht))\<close> by blast
+            moreover have \<open>n = n'\<close> 
+              using fields assms(1) f1 member \<open>ht \<in> set hts\<close> unfolding is_ht_specification_def by fastforce
+            ultimately have \<open>complies_ht M ?\<T>' \<Phi> (\<phi>, n, \<psi>)\<close> using fields by simp
+            then have 
+              \<open>(M \<Turnstile>\<^sub>M \<Phi> \<longleftrightarrow> ?\<T>' n M \<noteq> None) \<and>
+              (\<not> (fst M) \<Turnstile>\<^sub>L \<bottom>\<^sub>L \<longrightarrow> ?\<T>' n M \<noteq> None \<longrightarrow> \<not>the (?\<T>' n M) \<Turnstile>\<^sub>L \<bottom>\<^sub>L) \<and>
+              (M \<Turnstile>\<^sub>M \<phi> \<and> M \<Turnstile>\<^sub>M \<Phi> \<longrightarrow> the (\<M>* ?\<T>' (basic n) M) \<Turnstile>\<^sub>M \<psi>) \<and>
+              (M \<Turnstile>\<^sub>M \<phi> \<and> M \<Turnstile>\<^sub>M \<^bold>\<not> \<Phi> \<longrightarrow> M \<Turnstile>\<^sub>M \<psi>)\<close> by simp
+            moreover have \<open>n = fst s\<close> using f1 by simp
+            then have \<open>?\<T> n = ?\<T>' n\<close> using \<open>?\<T> (fst s) = ?\<T>' (fst s)\<close> by blast
+            moreover have \<open>\<M>* ?\<T> (basic n) M = \<M>* ?\<T>' (basic n) M\<close> 
+            proof (cases M)
+              case (Pair \<Sigma> \<Gamma>)
+              then have \<open>\<M>* ?\<T> (basic n) M = \<M>* ?\<T> (basic n) (\<Sigma>, \<Gamma>)\<close> by simp
+              also have \<open>\<M>* ?\<T> (basic n) (\<Sigma>, \<Gamma>) = (case ?\<T> n (\<Sigma>, \<Gamma>) of Some \<Sigma>' \<Rightarrow> Some (\<Sigma>', \<Gamma> - {\<psi> \<in> \<Gamma>. \<Sigma>' \<Turnstile>\<^sub>L \<psi>}) | _ \<Rightarrow> None)\<close> by simp
+              also have \<open>\<dots> = (case ?\<T>' n (\<Sigma>, \<Gamma>) of Some \<Sigma>' \<Rightarrow> Some (\<Sigma>', \<Gamma> - {\<psi> \<in> \<Gamma>. \<Sigma>' \<Turnstile>\<^sub>L \<psi>}) | _ \<Rightarrow> None)\<close> using \<open>?\<T> n = ?\<T>' n\<close> by simp
+              also have \<open>\<dots> = \<M>* ?\<T>' (basic n) (\<Sigma>, \<Gamma>)\<close> by simp
+              finally show \<open>\<M>* ?\<T> (basic n) M = \<M>* ?\<T>' (basic n) M\<close> using Pair by simp
+            qed
+            ultimately have 
+              \<open>(M \<Turnstile>\<^sub>M \<Phi> \<longleftrightarrow> ?\<T> n M \<noteq> None) \<and>
+              (\<not> (fst M) \<Turnstile>\<^sub>L \<bottom>\<^sub>L \<longrightarrow> ?\<T> n M \<noteq> None \<longrightarrow> \<not>the (?\<T> n M) \<Turnstile>\<^sub>L \<bottom>\<^sub>L) \<and>
+              (M \<Turnstile>\<^sub>M \<phi> \<and> M \<Turnstile>\<^sub>M \<Phi> \<longrightarrow> the (\<M>* ?\<T> (basic n) M) \<Turnstile>\<^sub>M \<psi>) \<and>
+              (M \<Turnstile>\<^sub>M \<phi> \<and> M \<Turnstile>\<^sub>M \<^bold>\<not> \<Phi> \<longrightarrow> M \<Turnstile>\<^sub>M \<psi>)\<close> by simp
+            then have \<open>complies_ht M ?\<T> \<Phi> (\<phi>, n, \<psi>)\<close> by simp
+            with \<open>n = n'\<close> show ?thesis using fields by simp
+          qed
+        qed
+      qed
+      moreover have \<open>\<forall>ht\<in>set hts. is_htb_basic ht\<close> 
+        using assms(1) f1 \<open>s \<in> set S\<close> unfolding is_ht_specification_def by simp
+      ultimately show ?thesis using f1 complies_hts_def by simp
+    qed
+    then show \<open>complies_hts s ?\<T> \<and> (\<forall>n. n \<notin> set (map fst S) \<longrightarrow> (\<forall>M. ?\<T> n M = None))\<close> by simp
+  qed
+qed
+
+\<comment> \<open>Definition used in proofs to put less strain on Isabelle's simplification methods.\<close>
+definition next_state_reqs where
+\<open>next_state_reqs M hts M' \<equiv> 
+  (\<not> fst M \<Turnstile>\<^sub>L \<bottom>\<^sub>L \<longrightarrow> \<not> fst M' \<Turnstile>\<^sub>L \<bottom>\<^sub>L) \<and> 
+  (snd M' = snd M - {\<psi> \<in> snd M. fst M' \<Turnstile>\<^sub>L \<psi>}) \<and> 
+  (\<forall>ht \<in> { ht \<in> set hts. M \<Turnstile>\<^sub>M pre ht }. M' \<Turnstile>\<^sub>M post ht)\<close>
+
+\<comment> \<open>If S is a valid specification, there exists a belief update function (model) that S complies to.\<close>
+lemma model_exists: \<open>is_ht_specification S \<Longrightarrow> \<exists>\<T>. complies S \<T>\<close>
+proof -
+  assume spec: \<open>is_ht_specification S\<close>
+  then have sat: \<open>satisfiable S\<close> unfolding is_ht_specification_def by simp
+  have \<open>\<forall>s\<in>set S. \<exists>\<T>. complies_hts s \<T>\<close> proof
+    fix s
+    assume \<open>s \<in> set S\<close>
+    show \<open>\<exists>\<T>. complies_hts s \<T>\<close> 
+    proof (cases s)
+      case f1: (fields n \<Phi> hts)
+      have \<open>\<exists>\<T>. complies_hts (n, \<Phi>, hts) \<T>\<close> 
+      proof
+        let ?\<T> = \<open>\<lambda>n M. if M \<Turnstile>\<^sub>M \<Phi> then Some (fst (SOME M'. next_state_reqs M hts M')) else None\<close>
+        have \<open>\<forall>ht\<in>set hts. is_htb_basic ht \<and> (\<forall>M. complies_ht M ?\<T> \<Phi> (the (htb_basic_unpack ht)))\<close>
+        proof
+          fix ht
+          assume \<open>ht \<in> set hts\<close>
+          show \<open>is_htb_basic ht \<and> (\<forall>M. complies_ht M ?\<T> \<Phi> (the (htb_basic_unpack ht)))\<close> 
+          proof
+            from spec show \<open>is_htb_basic ht\<close> 
+              using \<open>ht \<in> set hts\<close> \<open>s \<in> set S\<close> f1 unfolding is_ht_specification_def by simp
+            show \<open>\<forall>M. complies_ht M ?\<T> \<Phi> (the (htb_basic_unpack ht))\<close> 
+            proof
+              fix M
+              show \<open>complies_ht M ?\<T> \<Phi> (the (htb_basic_unpack ht))\<close>  
+              proof (cases \<open>the (htb_basic_unpack ht)\<close>)
+                case (fields \<phi> n' \<psi>)
+                moreover have \<open>complies_ht M ?\<T> \<Phi> (\<phi>, n, \<psi>)\<close>
+                proof (cases \<open>M \<Turnstile>\<^sub>M \<Phi>\<close>)
+                  case True
+                  then have nM: \<open>?\<T> n M = Some (fst (SOME M'. next_state_reqs M hts M'))\<close> by simp
+                  moreover from sat have 
+                    \<open>let (_, \<Phi>, hts) = s; sat_hts = { ht \<in> set hts. M \<Turnstile>\<^sub>M pre ht } in
+                      (M \<Turnstile>\<^sub>M \<Phi> \<longrightarrow> (\<exists>M'. (\<not> fst M \<Turnstile>\<^sub>L \<bottom>\<^sub>L \<longrightarrow> \<not> fst M' \<Turnstile>\<^sub>L \<bottom>\<^sub>L) \<and> 
+                        (snd M' = snd M - {\<psi> \<in> snd M. fst M' \<Turnstile>\<^sub>L \<psi>}) \<and> 
+                        (\<forall>ht \<in> sat_hts. M' \<Turnstile>\<^sub>M post ht))) \<and>
+                      (M \<Turnstile>\<^sub>M \<^bold>\<not> \<Phi> \<longrightarrow> (\<forall>ht \<in> sat_hts. M \<Turnstile>\<^sub>M post ht))\<close> 
+                    using \<open>s \<in> set S\<close> unfolding satisfiable_def by blast
+                  with f1 True have ex:
+                    \<open>\<exists>M'. next_state_reqs M hts M'\<close>
+                    unfolding next_state_reqs_def by simp
+                  have \<open>\<forall>M'. next_state_reqs M hts M' \<longrightarrow> \<not> (fst M) \<Turnstile>\<^sub>L \<bottom>\<^sub>L \<longrightarrow> ?\<T> n M \<noteq> None \<longrightarrow> \<not> fst M' \<Turnstile>\<^sub>L \<bottom>\<^sub>L\<close>
+                  proof
+                    fix M'
+                    show \<open>next_state_reqs M hts M' \<longrightarrow> \<not> (fst M) \<Turnstile>\<^sub>L \<bottom>\<^sub>L \<longrightarrow> ?\<T> n M \<noteq> None \<longrightarrow> \<not> fst M' \<Turnstile>\<^sub>L \<bottom>\<^sub>L\<close> 
+                    proof
+                      assume \<open>next_state_reqs M hts M'\<close>
+                      then show \<open>\<not> (fst M) \<Turnstile>\<^sub>L \<bottom>\<^sub>L \<longrightarrow> ?\<T> n M \<noteq> None \<longrightarrow> \<not> fst M' \<Turnstile>\<^sub>L \<bottom>\<^sub>L\<close> 
+                        unfolding next_state_reqs_def by simp
+                    qed
+                  qed
+                  with ex have \<open>\<not> (fst M) \<Turnstile>\<^sub>L \<bottom>\<^sub>L \<longrightarrow> ?\<T> n M \<noteq> None \<longrightarrow> \<not> fst (SOME M'. next_state_reqs M hts M') \<Turnstile>\<^sub>L \<bottom>\<^sub>L\<close>  
+                    using someI2[where ?P=\<open>next_state_reqs M hts\<close>] by blast
+                  moreover have \<open>\<forall>M'. next_state_reqs M hts M' \<longrightarrow> (M \<Turnstile>\<^sub>M \<phi> \<and> M \<Turnstile>\<^sub>M \<Phi> \<longrightarrow> M' \<Turnstile>\<^sub>M \<psi>)\<close>
+                  proof
+                    fix M'
+                    show \<open>next_state_reqs M hts M' \<longrightarrow> (M \<Turnstile>\<^sub>M \<phi> \<and> M \<Turnstile>\<^sub>M \<Phi> \<longrightarrow> M' \<Turnstile>\<^sub>M \<psi>)\<close> 
+                    proof
+                      assume \<open>next_state_reqs M hts M'\<close>
+                      with \<open>ht \<in> set hts\<close> have \<open>M \<Turnstile>\<^sub>M pre ht \<longrightarrow> M' \<Turnstile>\<^sub>M post ht\<close> unfolding next_state_reqs_def by simp
+                      moreover from \<open>is_htb_basic ht\<close> have \<open>pre ht = \<phi>\<close> 
+                        using fields unpack_sel(1) by fastforce
+                      moreover from \<open>is_htb_basic ht\<close> have \<open>post ht = \<psi>\<close> 
+                        using fields unpack_sel(2) by fastforce
+                      ultimately have \<open>M \<Turnstile>\<^sub>M \<phi> \<longrightarrow> M' \<Turnstile>\<^sub>M \<psi>\<close> by simp
+                      then show \<open>M \<Turnstile>\<^sub>M \<phi> \<and> M \<Turnstile>\<^sub>M \<Phi> \<longrightarrow> M' \<Turnstile>\<^sub>M \<psi>\<close> by simp
+                    qed
+                  qed
+                  with ex have \<open>(M \<Turnstile>\<^sub>M \<phi> \<and> M \<Turnstile>\<^sub>M \<Phi> \<longrightarrow> (SOME M'. next_state_reqs M hts M') \<Turnstile>\<^sub>M \<psi>)\<close>
+                    using someI2[where ?P=\<open>next_state_reqs M hts\<close>] by blast
+                  ultimately have 
+                    \<open>(M \<Turnstile>\<^sub>M \<Phi> \<longleftrightarrow> Some (fst (SOME M'. next_state_reqs M hts M')) \<noteq> None) \<and>
+                      (\<not> (fst M) \<Turnstile>\<^sub>L \<bottom>\<^sub>L \<longrightarrow> \<not> fst (SOME M'. next_state_reqs M hts M') \<Turnstile>\<^sub>L \<bottom>\<^sub>L) \<and>
+                      (M \<Turnstile>\<^sub>M \<phi> \<and> M \<Turnstile>\<^sub>M \<Phi> \<longrightarrow> (SOME M'. next_state_reqs M hts M') \<Turnstile>\<^sub>M \<psi>) \<and> 
+                      (M \<Turnstile>\<^sub>M \<phi> \<and> M \<Turnstile>\<^sub>M \<^bold>\<not> \<Phi> \<longrightarrow> M \<Turnstile>\<^sub>M \<psi>)\<close> 
+                    using True by auto
+                  moreover have \<open>(SOME M'. next_state_reqs M hts M') \<Turnstile>\<^sub>M \<psi> \<longrightarrow> the (\<M>* ?\<T> (basic n) M) \<Turnstile>\<^sub>M \<psi>\<close> 
+                  proof (cases M)
+                    case (Pair \<Sigma> \<Gamma>)
+                    show ?thesis 
+                    proof
+                      assume entails: \<open>(SOME M'. next_state_reqs M hts M') \<Turnstile>\<^sub>M \<psi>\<close>
+                      from Pair have \<open>\<forall>M'. next_state_reqs M hts M' \<longrightarrow> snd M' = (snd M - {\<psi> \<in> snd M. fst M' \<Turnstile>\<^sub>L \<psi>})\<close> 
+                        unfolding next_state_reqs_def by simp
+                      with ex have \<open>snd (SOME M'. next_state_reqs M hts M') = snd M - {\<psi> \<in> snd M. fst (SOME M'. next_state_reqs M hts M') \<Turnstile>\<^sub>L \<psi>}\<close>  
+                        using someI2[where ?P=\<open>next_state_reqs M hts\<close>] by blast
+                      with entails have \<open>(fst (SOME M'. next_state_reqs M hts M'), snd M - {\<psi> \<in> snd M. fst (SOME M'. next_state_reqs M hts M') \<Turnstile>\<^sub>L \<psi>}) \<Turnstile>\<^sub>M \<psi>\<close>
+                        by (metis prod.collapse)
+                      with nM Pair show \<open>the (\<M>* ?\<T> (basic n) M) \<Turnstile>\<^sub>M \<psi>\<close> by auto
+                    qed
+                  qed
+                  ultimately have 
+                    \<open>(M \<Turnstile>\<^sub>M \<Phi> \<longleftrightarrow> ?\<T> n M \<noteq> None) \<and>
+                      (\<not> (fst M) \<Turnstile>\<^sub>L \<bottom>\<^sub>L \<longrightarrow> ?\<T> n M \<noteq> None \<longrightarrow> \<not> the (?\<T> n M) \<Turnstile>\<^sub>L \<bottom>\<^sub>L) \<and>
+                      (M \<Turnstile>\<^sub>M \<phi> \<and> M \<Turnstile>\<^sub>M \<Phi> \<longrightarrow> the (\<M>* ?\<T> (basic n) M) \<Turnstile>\<^sub>M \<psi>) \<and> 
+                      (M \<Turnstile>\<^sub>M \<phi> \<and> M \<Turnstile>\<^sub>M \<^bold>\<not> \<Phi> \<longrightarrow> M \<Turnstile>\<^sub>M \<psi>)\<close> 
+                    using nM by simp
+                  then show ?thesis using complies_ht.simps by blast
+                next
+                  case False
+                  then have \<open>?\<T> n M = None\<close> by simp 
+                  then have \<open>M \<Turnstile>\<^sub>M \<phi> \<and> M \<Turnstile>\<^sub>M \<^bold>\<not> \<Phi> \<longrightarrow> M \<Turnstile>\<^sub>M \<psi>\<close> 
+                  proof -
+                    from sat have 
+                      \<open>let (_, \<Phi>, hts) = s; sat_hts = { ht \<in> set hts. M \<Turnstile>\<^sub>M pre ht } in
+                        (M \<Turnstile>\<^sub>M \<Phi> \<longrightarrow> (\<exists>M'. (\<not> fst M \<Turnstile>\<^sub>L \<bottom>\<^sub>L \<longrightarrow> \<not> fst M' \<Turnstile>\<^sub>L \<bottom>\<^sub>L) \<and> 
+                          (snd M' = snd M - {\<psi> \<in> snd M. fst M' \<Turnstile>\<^sub>L \<psi>}) \<and> 
+                          (\<forall>ht \<in> sat_hts. M' \<Turnstile>\<^sub>M post ht))) \<and>
+                        (M \<Turnstile>\<^sub>M \<^bold>\<not> \<Phi> \<longrightarrow> (\<forall>ht \<in> sat_hts. M \<Turnstile>\<^sub>M post ht))\<close> 
+                      using \<open>s \<in> set S\<close> unfolding satisfiable_def by blast
+                    then have \<open>\<forall>ht \<in> { ht \<in> set hts. M \<Turnstile>\<^sub>M pre ht }. M \<Turnstile>\<^sub>M post ht\<close> 
+                      using False f1 by simp
+                    with \<open>ht \<in> set hts\<close> have \<open>M \<Turnstile>\<^sub>M pre ht \<longrightarrow> M \<Turnstile>\<^sub>M post ht\<close> by simp
+                    moreover from \<open>is_htb_basic ht\<close> have \<open>pre ht = \<phi>\<close> 
+                      using fields unpack_sel(1) by fastforce
+                    moreover from \<open>is_htb_basic ht\<close> have \<open>post ht = \<psi>\<close> 
+                      using fields unpack_sel(2) by fastforce
+                    ultimately have \<open>M \<Turnstile>\<^sub>M \<phi> \<longrightarrow> M \<Turnstile>\<^sub>M \<psi>\<close> by simp
+                    then show ?thesis by simp
+                  qed
+                  with False show ?thesis by simp
+                qed
+                moreover from spec have \<open>n = n'\<close> 
+                  using \<open>s \<in> set S\<close> \<open>ht \<in> set hts\<close> f1 fields 
+                  unfolding is_ht_specification_def by fastforce
+                ultimately show ?thesis by metis
+              qed              
+            qed
+          qed
+        qed
+        then show \<open>complies_hts (n, \<Phi>, hts) ?\<T>\<close> unfolding complies_hts_def by simp
+      qed
+      with f1 show ?thesis by simp
+    qed
+  qed
+  with model_exists_disjoint \<open>is_ht_specification S\<close> show ?thesis .
+qed
+
+section \<open>Single agent program given by specification\<close>
 
 locale single_agent_program = single_agent + 
   fixes
     S :: ht_specification
   assumes
-    \<T>_complies: \<open>complies \<Pi> S \<T>\<close>
+    S_valid: \<open>is_ht_specification S\<close> and 
+    \<T>_complies: \<open>complies S \<T>\<close>
 
 context single_agent_program begin
 
-(* TODO import rules from specification *)
-section \<open>Proof System\<close>
+subsection \<open>Proof System\<close>
+
+\<comment> \<open>Derive (the) valid Hoare triples.\<close>
 
 inductive derive\<^sub>H :: \<open>hoare_triple \<Rightarrow> bool\<close> (\<open>\<turnstile>\<^sub>H\<close>) where
   \<comment> \<open>Agent specific rule import\<close>
+  import: \<open>(n, \<Phi>, hts) \<in> set S \<Longrightarrow> \<^bold>{ \<phi> \<^bold>} (basic n) \<^bold>{ \<psi> \<^bold>} \<in> set hts \<Longrightarrow> \<turnstile>\<^sub>H \<^bold>{ \<phi> \<^bold>} (basic n) \<^bold>{ \<psi> \<^bold>}\<close> |
   \<comment> \<open>Persistence of goals\<close>
-  persist:  \<open>a \<noteq> (drop \<Phi>) \<Longrightarrow> \<turnstile>\<^sub>H \<^bold>{ G \<Phi> \<^bold>} a \<^bold>{ (B \<Phi>) \<^bold>\<or> (G \<Phi>) \<^bold>}\<close> |
+  (*persist: \<open>\<not> is_drop a \<Longrightarrow> \<turnstile>\<^sub>H \<^bold>{ G \<Phi> \<^bold>} a \<^bold>{ (B \<Phi>) \<^bold>\<or> (G \<Phi>) \<^bold>}\<close> |*)
+  persist: \<open>\<not> is_drop a \<Longrightarrow> \<turnstile>\<^sub>H \<^bold>{ (G \<Phi>)  \<^bold>} a \<^bold>{ (B \<Phi>) \<^bold>\<or> (G \<Phi>) \<^bold>}\<close> |
   \<comment> \<open>Infeasible actions\<close>
-  inf:  \<open>\<turnstile>\<^sub>E ((\<phi>\<^sup>E) \<^bold>\<longrightarrow> \<^bold>\<not>(enabledb a)) \<Longrightarrow> \<turnstile>\<^sub>H \<^bold>{ \<phi> \<^bold>} a \<^bold>{ \<psi> \<^bold>}\<close> |
+  inf:  \<open>\<turnstile>\<^sub>E ((\<phi>\<^sup>E) \<^bold>\<longrightarrow> \<^bold>\<not>(enabledb a)) \<Longrightarrow> \<turnstile>\<^sub>H \<^bold>{ \<phi> \<^bold>} a \<^bold>{ \<phi> \<^bold>}\<close> |
   \<comment> \<open>Frame properties on beliefs for adopt and drop\<close>
   adoptB: \<open>\<turnstile>\<^sub>H \<^bold>{ B \<Phi> \<^bold>} (adopt \<psi>) \<^bold>{ B \<Phi> \<^bold>}\<close> |
   adoptNegB: \<open>\<turnstile>\<^sub>H \<^bold>{ \<^bold>\<not> (B \<Phi>) \<^bold>} (adopt \<psi>) \<^bold>{ \<^bold>\<not> (B \<Phi>) \<^bold>}\<close> |
   dropB: \<open>\<turnstile>\<^sub>H \<^bold>{ B \<Phi> \<^bold>} (drop \<psi>) \<^bold>{ B \<Phi> \<^bold>}\<close> |
   dropNegB: \<open>\<turnstile>\<^sub>H \<^bold>{ \<^bold>\<not> (B \<Phi>) \<^bold>} (drop \<psi>) \<^bold>{ \<^bold>\<not> (B \<Phi>) \<^bold>}\<close> |
   \<comment> \<open>Effects of adopt\<close>
-  adoptBG: \<open>\<not> \<turnstile>\<^sub>P (\<^bold>\<not> \<Phi>) \<Longrightarrow> \<turnstile>\<^sub>H \<^bold>{ B \<Phi> \<^bold>} (adopt \<Phi>) \<^bold>{ G \<Phi> \<^bold>}\<close> |
+  adoptBG: \<open>\<not> {} \<Turnstile>\<^sub>P (\<^bold>\<not> \<Phi>) \<Longrightarrow> \<turnstile>\<^sub>H \<^bold>{ \<^bold>\<not> (B \<Phi>) \<^bold>} (adopt \<Phi>) \<^bold>{ G \<Phi> \<^bold>}\<close> |
   \<comment> \<open>Non-effect of adopt\<close>
   adoptG: \<open>\<turnstile>\<^sub>H \<^bold>{ G \<Phi> \<^bold>} (adopt \<psi>) \<^bold>{ G \<Phi> \<^bold>}\<close> |
-  adoptNegG: \<open>\<not> \<turnstile>\<^sub>P \<psi> \<^bold>\<longrightarrow> \<Phi> \<Longrightarrow> \<turnstile>\<^sub>H \<^bold>{ \<^bold>\<not> (G \<Phi>) \<^bold>} (adopt \<psi>) \<^bold>{ \<^bold>\<not> (G \<Phi>) \<^bold>}\<close> |
+  adoptNegG: \<open>\<not> {} \<Turnstile>\<^sub>P \<psi> \<^bold>\<longrightarrow> \<Phi> \<Longrightarrow> \<turnstile>\<^sub>H \<^bold>{ \<^bold>\<not> (G \<Phi>) \<^bold>} (adopt \<psi>) \<^bold>{ \<^bold>\<not> (G \<Phi>) \<^bold>}\<close> |
   \<comment> \<open>Effects of drop\<close>
-  dropG: \<open>\<turnstile>\<^sub>P \<Phi> \<^bold>\<longrightarrow> \<psi> \<Longrightarrow> \<turnstile>\<^sub>H \<^bold>{ G \<Phi> \<^bold>} (drop \<psi>) \<^bold>{ \<^bold>\<not> (G \<Phi>) \<^bold>}\<close> |
+  dropG: \<open>{} \<Turnstile>\<^sub>P \<Phi> \<^bold>\<longrightarrow> \<psi> \<Longrightarrow> \<turnstile>\<^sub>H \<^bold>{ G \<Phi> \<^bold>} (drop \<psi>) \<^bold>{ \<^bold>\<not> (G \<Phi>) \<^bold>}\<close> |
   \<comment> \<open>Non-effects of drop\<close>
   dropNegG: \<open>\<turnstile>\<^sub>H \<^bold>{ \<^bold>\<not>(G \<Phi>) \<^bold>} (drop \<psi>) \<^bold>{ \<^bold>\<not>(G \<Phi>) \<^bold>}\<close> |
   dropGCon: \<open>\<turnstile>\<^sub>H \<^bold>{ \<^bold>\<not>(G (\<Phi> \<^bold>\<and> \<psi>)) \<^bold>\<and> (G \<Phi>) \<^bold>} (drop \<psi>) \<^bold>{ G \<Phi> \<^bold>}\<close> |
@@ -65,60 +346,314 @@ inductive derive\<^sub>H :: \<open>hoare_triple \<Rightarrow> bool\<close> (\<op
   rCon: \<open>\<turnstile>\<^sub>H \<^bold>{ \<phi>\<^sub>1 \<^bold>} a \<^bold>{ \<psi>\<^sub>1 \<^bold>} \<Longrightarrow> \<turnstile>\<^sub>H \<^bold>{ \<phi>\<^sub>2 \<^bold>} a \<^bold>{ \<psi>\<^sub>2 \<^bold>} \<Longrightarrow> \<turnstile>\<^sub>H \<^bold>{ \<phi>\<^sub>1 \<^bold>\<and> \<phi>\<^sub>2 \<^bold>} a \<^bold>{ \<psi>\<^sub>1 \<^bold>\<and> \<psi>\<^sub>2 \<^bold>}\<close> |
   rDis: \<open>\<turnstile>\<^sub>H \<^bold>{ \<phi>\<^sub>1 \<^bold>} a \<^bold>{ \<psi> \<^bold>} \<Longrightarrow> \<turnstile>\<^sub>H \<^bold>{ \<phi>\<^sub>2 \<^bold>} a \<^bold>{ \<psi> \<^bold>} \<Longrightarrow> \<turnstile>\<^sub>H \<^bold>{ \<phi>\<^sub>1 \<^bold>\<or> \<phi>\<^sub>2 \<^bold>} a \<^bold>{ \<psi> \<^bold>}\<close>
 
+\<comment> \<open>A proof of a Hoare triple ensures validity.\<close>
+\<comment> \<open>Induction over each rule.\<close>
 theorem soundness\<^sub>H: \<open>\<turnstile>\<^sub>H H \<Longrightarrow> \<Turnstile>\<^sub>H H\<close> 
-  sorry
+proof (induct rule: derive\<^sub>H.induct)
+  case (import n \<Phi> hts \<phi> \<psi>)
+  let ?a = \<open>basic n\<close> 
+  let ?ht = \<open>\<^bold>{ \<phi> \<^bold>} ?a \<^bold>{ \<psi> \<^bold>}\<close>
+  have \<open>\<forall>s\<in>set S. complies_hts s \<T>\<close> using \<T>_complies unfolding complies_def by simp
+  with import(1) have \<open>\<forall>ht\<in>set hts. is_htb_basic ht \<and> (\<forall>M. complies_ht M \<T> \<Phi> (the (htb_basic_unpack ht)))\<close> 
+    unfolding complies_hts_def by auto
+  with bspec have \<open>is_htb_basic ?ht \<and> (\<forall>M. complies_ht M \<T> \<Phi> (the (htb_basic_unpack ?ht)))\<close> 
+    using import(2) .
+  then have **: 
+    \<open>\<forall>M. (M \<Turnstile>\<^sub>M \<Phi> \<longleftrightarrow> \<T> n M \<noteq> None) \<and>
+         (M \<Turnstile>\<^sub>M \<phi> \<and> M \<Turnstile>\<^sub>M \<Phi> \<longrightarrow> the (\<M>* \<T> (basic n) M) \<Turnstile>\<^sub>M \<psi>) \<and>
+         (M \<Turnstile>\<^sub>M \<phi> \<and> M \<Turnstile>\<^sub>M \<^bold>\<not> \<Phi> \<longrightarrow> M \<Turnstile>\<^sub>M \<psi>)\<close>
+    by simp
+  have *:   (* Could be optimized/cleaned I think... *)
+    \<open>\<forall>M. (M \<Turnstile>\<^sub>M \<Phi> \<longleftrightarrow> \<T> n M \<noteq> None) \<and>
+         (M \<Turnstile>\<^sub>M \<phi> \<and> M \<Turnstile>\<^sub>M \<Phi> \<longrightarrow> the (\<M> ?a M) \<Turnstile>\<^sub>M \<psi>) \<and>
+         (M \<Turnstile>\<^sub>M \<phi> \<and> M \<Turnstile>\<^sub>M \<^bold>\<not> \<Phi> \<longrightarrow> M \<Turnstile>\<^sub>M \<psi>)\<close>
+  proof 
+    fix M
+    show \<open>(M \<Turnstile>\<^sub>M \<Phi> \<longleftrightarrow> \<T> n M \<noteq> None) \<and>
+          (M \<Turnstile>\<^sub>M \<phi> \<and> M \<Turnstile>\<^sub>M \<Phi> \<longrightarrow> the (\<M> ?a M) \<Turnstile>\<^sub>M \<psi>) \<and>
+          (M \<Turnstile>\<^sub>M \<phi> \<and> M \<Turnstile>\<^sub>M \<^bold>\<not> \<Phi> \<longrightarrow> M \<Turnstile>\<^sub>M \<psi>)\<close>
+    proof (cases M)
+      case (Pair \<Sigma> \<Gamma>)
+      with ** have \<open>((\<Sigma>, \<Gamma>) \<Turnstile>\<^sub>M \<Phi> \<longleftrightarrow> \<T> n M \<noteq> None) \<and>
+         ((\<Sigma>, \<Gamma>) \<Turnstile>\<^sub>M \<phi> \<and> (\<Sigma>, \<Gamma>) \<Turnstile>\<^sub>M \<Phi> \<longrightarrow> the (\<M>* \<T> (basic n) M) \<Turnstile>\<^sub>M \<psi>) \<and>
+         ((\<Sigma>, \<Gamma>) \<Turnstile>\<^sub>M \<phi> \<and> (\<Sigma>, \<Gamma>) \<Turnstile>\<^sub>M \<^bold>\<not> \<Phi> \<longrightarrow> (\<Sigma>, \<Gamma>) \<Turnstile>\<^sub>M \<psi>)\<close> by simp
+      then show ?thesis using Pair by simp
+    qed
+  qed
+  have \<open>\<forall>M. (M \<Turnstile>\<^sub>E (\<phi>\<^sup>E) \<^bold>\<and> (enabledb ?a) \<longrightarrow> the (\<M> ?a M) \<Turnstile>\<^sub>M \<psi>) \<and> (M \<Turnstile>\<^sub>E (\<phi>\<^sup>E) \<^bold>\<and> \<^bold>\<not>(enabledb ?a) \<longrightarrow> M \<Turnstile>\<^sub>M \<psi>)\<close>
+  proof
+    fix M
+    from * have 
+      \<open>(M \<Turnstile>\<^sub>M \<phi> \<and> M \<Turnstile>\<^sub>M \<Phi> \<longrightarrow> the (\<M> ?a M) \<Turnstile>\<^sub>M \<psi>) \<and>
+       (M \<Turnstile>\<^sub>M \<phi> \<and> M \<Turnstile>\<^sub>M \<^bold>\<not> \<Phi> \<longrightarrow> M \<Turnstile>\<^sub>M \<psi>)\<close> 
+      by blast
+    moreover have \<open>M \<Turnstile>\<^sub>E (enabledb ?a) \<longleftrightarrow> M \<Turnstile>\<^sub>M \<Phi>\<close> 
+    proof (cases M)
+      case (Pair \<Sigma> \<Gamma>)
+      with * have \<open>(\<Sigma>, \<Gamma>) \<Turnstile>\<^sub>M \<Phi> \<longleftrightarrow> \<T> n (\<Sigma>, \<Gamma>) \<noteq> None\<close> by blast
+      moreover have \<open>\<T> n (\<Sigma>, \<Gamma>) \<noteq> None \<longrightarrow> \<M> (basic n) (\<Sigma>, \<Gamma>) \<noteq> None\<close> by auto
+      moreover have \<open>\<dots> \<longrightarrow> (\<Sigma>, \<Gamma>) \<Turnstile>\<^sub>E (enabledb ?a)\<close> by simp
+      ultimately show ?thesis using Pair by auto
+    qed
+    ultimately have 
+      \<open>(M \<Turnstile>\<^sub>M \<phi> \<and> M \<Turnstile>\<^sub>E (enabledb ?a) \<longrightarrow> the (\<M> ?a M) \<Turnstile>\<^sub>M \<psi>) \<and> 
+       (M \<Turnstile>\<^sub>M \<phi> \<and> M \<Turnstile>\<^sub>E \<^bold>\<not> (enabledb ?a) \<longrightarrow> M \<Turnstile>\<^sub>M \<psi>)\<close> by simp
+    then show \<open>(M \<Turnstile>\<^sub>E (\<phi>\<^sup>E) \<^bold>\<and> (enabledb ?a) \<longrightarrow> the (\<M> ?a M) \<Turnstile>\<^sub>M \<psi>) \<and> (M \<Turnstile>\<^sub>E (\<phi>\<^sup>E) \<^bold>\<and> \<^bold>\<not>(enabledb ?a) \<longrightarrow> M \<Turnstile>\<^sub>M \<psi>)\<close>  
+      using transfer_semantics\<^sub>M by simp
+  qed
+  then show ?case by simp
+next
+  case (persist a \<Phi>)
+  have \<open>\<forall>M. (M \<Turnstile>\<^sub>M (G \<Phi>) \<and> M \<Turnstile>\<^sub>E (enabledb a) \<longrightarrow> the (\<M> a M) \<Turnstile>\<^sub>M (B \<Phi>) \<^bold>\<or> (G \<Phi>)) \<and> 
+            (M \<Turnstile>\<^sub>M (G \<Phi>) \<and> M \<Turnstile>\<^sub>E \<^bold>\<not>(enabledb a) \<longrightarrow> M \<Turnstile>\<^sub>M (B \<Phi>) \<^bold>\<or> (G \<Phi>))\<close>
+  proof
+    fix M
+    show \<open>(M \<Turnstile>\<^sub>M (G \<Phi>) \<and> M \<Turnstile>\<^sub>E (enabledb a) \<longrightarrow> the (\<M> a M) \<Turnstile>\<^sub>M (B \<Phi>) \<^bold>\<or> (G \<Phi>)) \<and> 
+          (M \<Turnstile>\<^sub>M (G \<Phi>) \<and> M \<Turnstile>\<^sub>E \<^bold>\<not>(enabledb a) \<longrightarrow> M \<Turnstile>\<^sub>M (B \<Phi>) \<^bold>\<or> (G \<Phi>))\<close>
+    proof (cases M)
+      case (Pair \<Sigma> \<Gamma>)
+      show ?thesis
+      proof
+        show \<open>M \<Turnstile>\<^sub>M (G \<Phi>) \<and> M \<Turnstile>\<^sub>E (enabledb a) \<longrightarrow> the (\<M> a M) \<Turnstile>\<^sub>M (B \<Phi>) \<^bold>\<or> (G \<Phi>)\<close> 
+        proof
+          assume asm: \<open>M \<Turnstile>\<^sub>M (G \<Phi>) \<and> M \<Turnstile>\<^sub>E (enabledb a)\<close>
+          with Pair have notNone: \<open>\<M> a (\<Sigma>, \<Gamma>) \<noteq> None\<close> by simp
+          show \<open>the (\<M> a M) \<Turnstile>\<^sub>M (B \<Phi>) \<^bold>\<or> (G \<Phi>)\<close> 
+          proof (cases a)
+            case (basic n)
+            with notNone have \<open>\<M> (basic n) (\<Sigma>, \<Gamma>) \<noteq> None\<close> by simp
+            then obtain \<Sigma>' where \<Sigma>': \<open>\<T> n (\<Sigma>, \<Gamma>) = Some \<Sigma>'\<close> by fastforce
+            then have mst_unfold: \<open>\<M> (basic n) (\<Sigma>, \<Gamma>) = Some (\<Sigma>', \<Gamma> - {\<psi> \<in> \<Gamma>. \<Sigma>' \<Turnstile>\<^sub>L \<psi>})\<close>
+                              (is \<open>\<M> (basic n) (\<Sigma>, \<Gamma>) = Some (\<Sigma>', ?\<Gamma>')\<close>) 
+              by simp
+            then show ?thesis 
+            proof (cases \<open>\<Sigma>' \<Turnstile>\<^sub>L \<Phi>\<close>)
+              case True
+              then have \<open>(\<Sigma>', ?\<Gamma>') \<Turnstile>\<^sub>M (B \<Phi>) \<^bold>\<or> (G \<Phi>)\<close> by auto
+              with mst_unfold show ?thesis using basic Pair by simp
+            next
+              case False
+              moreover from asm have \<open>(\<Sigma>, \<Gamma>) \<Turnstile>\<^sub>M G \<Phi>\<close> using Pair by simp
+              ultimately have \<open>(\<Sigma>', ?\<Gamma>') \<Turnstile>\<^sub>M G \<Phi>\<close> by auto
+              with mst_unfold show ?thesis using basic Pair by simp
+            qed
+          next
+            case (adopt \<Phi>')
+            have \<open>\<M> (adopt \<Phi>') (\<Sigma>, \<Gamma>) = (if \<not> {} \<Turnstile>\<^sub>L \<^bold>\<not> \<Phi>' \<and> \<not> \<Sigma> \<Turnstile>\<^sub>L \<Phi>' then Some (\<Sigma>, \<Gamma> \<union> {\<Phi>'}) else None)\<close> 
+              by simp
+            with notNone have \<open>\<M> (adopt \<Phi>') (\<Sigma>, \<Gamma>) = Some (\<Sigma>, \<Gamma> \<union> {\<Phi>'})\<close> using adopt by metis
+            then show ?thesis using adopt Pair asm by simp
+          next 
+            case (drop \<psi>)  
+            with persist show ?thesis by simp
+          qed
+        qed
+      qed simp 
+    qed
+  qed
+  then show ?case by simp
+next
+  case (inf \<phi> a)
+  then have \<open>\<forall>M. \<nabla>M \<longrightarrow> M \<Turnstile>\<^sub>E (\<phi>\<^sup>E) \<^bold>\<longrightarrow> \<^bold>\<not> (enabledb a)\<close> using soundness\<^sub>E by blast
+  then have \<open>\<forall>M. \<nabla>M \<longrightarrow> (M \<Turnstile>\<^sub>E (\<phi>\<^sup>E) \<^bold>\<and>  (enabledb a) \<longrightarrow> the (\<M> a M) \<Turnstile>\<^sub>M \<phi>) \<and> 
+                         (M \<Turnstile>\<^sub>E (\<phi>\<^sup>E) \<^bold>\<and> \<^bold>\<not>(enabledb a) \<longrightarrow> M \<Turnstile>\<^sub>M \<phi>)\<close>
+    using transfer_semantics\<^sub>M by auto
+  then show ?case by auto
+next
+  case (adoptBG \<Phi>)
+  let ?\<phi> = \<open>\<^bold>\<not> (B \<Phi>)\<close> and ?\<psi> = \<open>G \<Phi>\<close> and ?a = \<open>adopt \<Phi>\<close>
+  have \<open>\<forall>M. \<nabla>M \<longrightarrow> 
+        (M \<Turnstile>\<^sub>E (?\<phi>\<^sup>E) \<^bold>\<and>  (enabledb ?a) \<longrightarrow> the (\<M> ?a M) \<Turnstile>\<^sub>M ?\<psi>) \<and> 
+        (M \<Turnstile>\<^sub>E (?\<phi>\<^sup>E) \<^bold>\<and> \<^bold>\<not>(enabledb ?a) \<longrightarrow> M \<Turnstile>\<^sub>M ?\<psi>)\<close>
+  proof
+    fix M 
+    have \<open>\<nabla>M \<longrightarrow> M \<Turnstile>\<^sub>E (?\<phi>\<^sup>E) \<longrightarrow> the (\<M> ?a M) \<Turnstile>\<^sub>M ?\<psi> \<and> M \<Turnstile>\<^sub>E enabledb ?a\<close>
+    proof
+      assume \<open>\<nabla> M\<close>
+      show \<open>M \<Turnstile>\<^sub>E (?\<phi>\<^sup>E) \<longrightarrow> the (\<M> ?a M) \<Turnstile>\<^sub>M ?\<psi> \<and> M \<Turnstile>\<^sub>E enabledb ?a\<close>
+      proof
+        assume \<open>M \<Turnstile>\<^sub>E (?\<phi>\<^sup>E)\<close>
+        show \<open>the (\<M> ?a M) \<Turnstile>\<^sub>M ?\<psi> \<and> M \<Turnstile>\<^sub>E enabledb ?a\<close>
+        proof
+          from \<open>M \<Turnstile>\<^sub>E (?\<phi>\<^sup>E)\<close> show \<open>M \<Turnstile>\<^sub>E enabledb ?a\<close> using adoptBG by (cases M) simp
+          with \<open>M \<Turnstile>\<^sub>E (?\<phi>\<^sup>E)\<close> adoptBG have s: \<open>\<M> ?a M = Some (fst M, snd M \<union> {\<Phi>})\<close> by (cases M) simp
+          then have \<open>\<exists>\<gamma>\<in>snd (the (\<M> ?a M)). {} \<Turnstile>\<^sub>L \<gamma> \<^bold>\<longrightarrow> \<Phi>\<close> by simp
+          moreover {
+            from s have \<open>fst (the (\<M> ?a M)) = fst M\<close> by simp
+            moreover have \<open>\<not> fst M \<Turnstile>\<^sub>L \<Phi>\<close> using \<open>M \<Turnstile>\<^sub>E (?\<phi>\<^sup>E)\<close> by (cases M) simp
+            ultimately have \<open>\<not> fst (the (\<M> ?a M)) \<Turnstile>\<^sub>L \<Phi>\<close> by simp
+          }
+          ultimately show \<open>the (\<M> ?a M) \<Turnstile>\<^sub>M ?\<psi>\<close> 
+            using semantics\<^sub>M'.simps(2)[where \<Sigma>=\<open>fst (the (\<M> ?a M))\<close> and \<Gamma>=\<open>snd (the (\<M> ?a M))\<close>] 
+            by simp
+        qed
+      qed
+    qed
+    then show 
+      \<open>\<nabla>M \<longrightarrow>
+        (M \<Turnstile>\<^sub>E (?\<phi>\<^sup>E) \<^bold>\<and>  (enabledb ?a) \<longrightarrow> the (\<M> ?a M) \<Turnstile>\<^sub>M ?\<psi>) \<and> 
+        (M \<Turnstile>\<^sub>E (?\<phi>\<^sup>E) \<^bold>\<and> \<^bold>\<not>(enabledb ?a) \<longrightarrow> M \<Turnstile>\<^sub>M ?\<psi>)\<close> 
+      by auto
+  qed
+  then show ?case by simp
+next
+  case (dropGCon \<Phi> \<psi>)
+  let ?\<phi> = \<open>\<^bold>\<not> (G (\<Phi> \<^bold>\<and> \<psi>)) \<^bold>\<and> (G \<Phi>)\<close> and ?\<psi> = \<open>G \<Phi>\<close> and ?a = \<open>drop \<psi>\<close>
+  have \<open>\<forall>M. \<nabla>M \<longrightarrow> (M \<Turnstile>\<^sub>M ?\<phi> \<longrightarrow> the (\<M> ?a M) \<Turnstile>\<^sub>M ?\<psi>)\<close> 
+  proof
+    fix M
+    show \<open>\<nabla>M \<longrightarrow> (M \<Turnstile>\<^sub>M ?\<phi> \<longrightarrow> the (\<M> ?a M) \<Turnstile>\<^sub>M ?\<psi>)\<close>
+    proof
+      assume \<open>\<nabla>M\<close>
+      show \<open>M \<Turnstile>\<^sub>M ?\<phi> \<longrightarrow> the (\<M> ?a M) \<Turnstile>\<^sub>M ?\<psi>\<close>
+      proof
+        assume \<open>M \<Turnstile>\<^sub>M ?\<phi>\<close>      
+        with dropGCon have pre:
+          \<open>\<not> fst M \<Turnstile>\<^sub>L \<Phi> \<and> 
+           \<not> (\<exists>\<gamma>\<in>snd M. {} \<Turnstile>\<^sub>L \<gamma> \<^bold>\<longrightarrow> (\<Phi> \<^bold>\<and> \<psi>)) \<and> 
+              (\<exists>\<gamma>\<in>snd M. {} \<Turnstile>\<^sub>L \<gamma> \<^bold>\<longrightarrow> \<Phi>)\<close>  
+          by (cases M) auto
+        moreover from pre obtain \<gamma> where gamma: \<open>\<gamma> \<in> snd M \<and> {} \<Turnstile>\<^sub>L \<gamma> \<^bold>\<longrightarrow> \<Phi>\<close> by auto
+        moreover have aM: \<open>\<M> ?a M = Some (fst M, snd M - {\<gamma> \<in> snd M. {\<gamma>} \<Turnstile>\<^sub>L \<psi>})\<close> (is \<open>\<dots> = Some ?M'\<close>) 
+          by (cases M) simp
+        ultimately have \<open>\<not> fst ?M' \<Turnstile>\<^sub>L \<Phi>\<close> by simp
+        moreover from pre gamma have \<open>\<not> {\<gamma>} \<Turnstile>\<^sub>L \<Phi> \<^bold>\<and> \<psi>\<close> by auto
+        with gamma have \<open>\<exists>\<gamma>\<in>snd ?M'. {} \<Turnstile>\<^sub>L \<gamma> \<^bold>\<longrightarrow> \<Phi>\<close> by auto
+        ultimately show \<open>the (\<M> ?a M) \<Turnstile>\<^sub>M ?\<psi>\<close> using aM by simp
+      qed
+    qed
+  qed
+  then show ?case by simp
+next
+  case (rCondAct \<phi> \<psi> a \<phi>')
+  have \<open>\<forall> s \<in> Agent. \<forall>i. ((\<phi>\<^bold>[s i\<^bold>]\<^sub>M) \<and> (\<psi> \<triangleright> do a) = (act_nth s i) \<longrightarrow> (\<phi>'\<^bold>[s (i+1)\<^bold>]\<^sub>M))\<close>
+  proof
+    fix s
+    assume \<open>s \<in> Agent\<close>
+    show \<open>\<forall>i. ((\<phi>\<^bold>[s i\<^bold>]\<^sub>M) \<and> (\<psi> \<triangleright> do a) = (act_nth s i) \<longrightarrow> (\<phi>'\<^bold>[s (i+1)\<^bold>]\<^sub>M))\<close>
+    proof
+      fix i
+      have \<open>\<nabla> (st_nth s i)\<close> using is_mst_trace \<open>s \<in> Agent\<close> .
+      with rCondAct have a:
+        \<open>((\<phi> \<^bold>\<and> \<^bold>\<not>\<psi>) \<^bold>\<longrightarrow> \<phi>')\<^bold>[s i\<^bold>]\<^sub>M\<close> 
+        \<open>(st_nth s i \<Turnstile>\<^sub>E ((\<phi> \<^bold>\<and> \<psi>)\<^sup>E) \<^bold>\<and>  (enabledb a) \<longrightarrow> the (\<M> a (st_nth s i)) \<Turnstile>\<^sub>M \<phi>') \<and>
+         (st_nth s i \<Turnstile>\<^sub>E ((\<phi> \<^bold>\<and> \<psi>)\<^sup>E) \<^bold>\<and> \<^bold>\<not>(enabledb a) \<longrightarrow> st_nth s i \<Turnstile>\<^sub>M \<phi>')\<close>
+        using soundness\<^sub>M semantics\<^sub>H.simps(1) by blast+
+      show \<open>(\<phi>\<^bold>[s i\<^bold>]\<^sub>M) \<and> (\<psi> \<triangleright> do a) = (act_nth s i) \<longrightarrow> (\<phi>'\<^bold>[s (i+1)\<^bold>]\<^sub>M)\<close> 
+      proof
+        assume pre: \<open>st_nth s i \<Turnstile>\<^sub>M \<phi> \<and> (\<psi>, a) = act_nth s i\<close>
+        then have bact: \<open>(\<psi>, a) = act_nth s i\<close> by simp
+        show \<open>\<phi>'\<^bold>[s (i+1)\<^bold>]\<^sub>M\<close>
+        proof (cases \<open>(st_nth s i) \<rightarrow>(\<psi>, a) (st_nth s (i+1))\<close>)
+          case True
+          then have \<open>st_nth s i \<Turnstile>\<^sub>M \<psi>\<close> unfolding transition_def by simp
+          with pre have \<open>st_nth s i \<Turnstile>\<^sub>E ((\<phi> \<^bold>\<and> \<psi>)\<^sup>E)\<close> using transfer_semantics\<^sub>M by simp
+          moreover from True have \<open>\<M> a (st_nth s i) \<noteq> None\<close> unfolding transition_def by simp
+          moreover from this have \<open>st_nth s i \<Turnstile>\<^sub>E enabledb a\<close> by simp
+          ultimately show ?thesis using \<M>_suc_state \<open>s \<in> Agent\<close> bact a(2) by auto
+        next
+          case False
+          moreover from \<open>s \<in> Agent\<close> have \<open>is_trace s\<close> unfolding Agent_def by simp
+          ultimately have \<open>st_nth s i = st_nth s (i+1)\<close> using not_transition_eq bact by simp
+          moreover from \<open>is_trace s\<close> have 
+            \<open>let (M, M', \<phi>, a) = (st_nth s i, st_nth s (i + 1), act_nth s i) in 
+              (\<phi>, a) \<in> \<Pi> \<and> ((M \<rightarrow>(\<phi>, a) M') \<or> \<M> a M = None \<and> M = M')\<close> 
+            unfolding is_trace_def by simp
+          with False bact have \<open>\<M> a (st_nth s i) = None\<close> by auto
+          ultimately show ?thesis using a pre transfer_semantics\<^sub>M by auto
+        qed
+      qed
+    qed
+  qed
+  then show ?case by simp
+next
+  case (rImp \<phi>' \<phi> a \<psi> \<psi>')
+  have 
+    \<open>\<forall>M. \<nabla>M \<longrightarrow>
+      (M \<Turnstile>\<^sub>M \<phi>' \<and> M \<Turnstile>\<^sub>E (enabledb a) \<longrightarrow> the (\<M> a M) \<Turnstile>\<^sub>M \<psi>') \<and> 
+      (M \<Turnstile>\<^sub>M \<phi>' \<and> M \<Turnstile>\<^sub>E \<^bold>\<not>(enabledb a) \<longrightarrow> M \<Turnstile>\<^sub>M \<psi>')\<close> 
+  proof
+    fix M
+    show \<open>\<nabla>M \<longrightarrow>
+      (M \<Turnstile>\<^sub>M \<phi>' \<and> M \<Turnstile>\<^sub>E (enabledb a) \<longrightarrow> the (\<M> a M) \<Turnstile>\<^sub>M \<psi>') \<and> 
+      (M \<Turnstile>\<^sub>M \<phi>' \<and> M \<Turnstile>\<^sub>E \<^bold>\<not>(enabledb a) \<longrightarrow> M \<Turnstile>\<^sub>M \<psi>')\<close>
+    proof
+      assume \<open>\<nabla>M\<close>
+      show 
+        \<open>(M \<Turnstile>\<^sub>M \<phi>' \<and> M \<Turnstile>\<^sub>E (enabledb a) \<longrightarrow> the (\<M> a M) \<Turnstile>\<^sub>M \<psi>') \<and> 
+         (M \<Turnstile>\<^sub>M \<phi>' \<and> M \<Turnstile>\<^sub>E \<^bold>\<not>(enabledb a) \<longrightarrow> M \<Turnstile>\<^sub>M \<psi>')\<close> 
+      proof
+        show \<open>M \<Turnstile>\<^sub>M \<phi>' \<and> M \<Turnstile>\<^sub>E (enabledb a) \<longrightarrow> the (\<M> a M) \<Turnstile>\<^sub>M \<psi>'\<close> 
+        proof
+          assume pre: \<open>M \<Turnstile>\<^sub>M \<phi>' \<and> M \<Turnstile>\<^sub>E (enabledb a)\<close>
+          moreover from rImp have \<open>M \<Turnstile>\<^sub>M \<phi> \<and> M \<Turnstile>\<^sub>E (enabledb a) \<longrightarrow> the (\<M> a M) \<Turnstile>\<^sub>M \<psi>\<close> 
+            using \<open>\<nabla>M\<close> transfer_semantics\<^sub>M semantics\<^sub>H.simps(1) semantics\<^sub>P.simps(5) by blast
+          moreover from soundness\<^sub>M  have \<open>M \<Turnstile>\<^sub>M \<phi>' \<^bold>\<longrightarrow> \<phi>\<close> 
+            using \<open>\<nabla>M\<close> rImp(1) by blast
+          moreover have \<open>\<nabla> (the (\<M> a M))\<close> using \<open>\<nabla>M\<close> \<M>_preserves_mst pre by (cases M) simp
+          with soundness\<^sub>M  have \<open>the (\<M> a M) \<Turnstile>\<^sub>M \<psi> \<^bold>\<longrightarrow> \<psi>'\<close> using rImp(4) by blast
+          ultimately show \<open>the (\<M> a M) \<Turnstile>\<^sub>M \<psi>'\<close> by simp
+        qed
+        show \<open>M \<Turnstile>\<^sub>M \<phi>' \<and> M \<Turnstile>\<^sub>E \<^bold>\<not>(enabledb a) \<longrightarrow> M \<Turnstile>\<^sub>M \<psi>'\<close>
+        proof
+          assume pre: \<open>M \<Turnstile>\<^sub>M \<phi>' \<and> M \<Turnstile>\<^sub>E \<^bold>\<not>(enabledb a)\<close>
+          from rImp(3) have \<open>M \<Turnstile>\<^sub>M \<phi> \<and> M \<Turnstile>\<^sub>E \<^bold>\<not>(enabledb a) \<longrightarrow> M \<Turnstile>\<^sub>M \<psi>\<close> 
+            using \<open>\<nabla>M\<close> transfer_semantics\<^sub>M semantics\<^sub>H.simps(1) semantics\<^sub>P.simps(5) by blast
+          moreover from soundness\<^sub>M  have \<open>M \<Turnstile>\<^sub>M \<phi>' \<^bold>\<longrightarrow> \<phi>\<close> 
+            using \<open>\<nabla>M\<close> rImp(1) by blast
+          moreover from soundness\<^sub>M  have \<open>M \<Turnstile>\<^sub>M \<psi> \<^bold>\<longrightarrow> \<psi>'\<close>
+            using \<open>\<nabla>M\<close> rImp(4) by blast
+          ultimately show \<open>M \<Turnstile>\<^sub>M \<psi>'\<close> using pre by simp
+        qed
+      qed
+    qed
+  qed
+  with transfer_semantics\<^sub>M show ?case by simp
+next
+  case (rDis \<phi>\<^sub>1 a \<psi> \<phi>\<^sub>2)
+  have 
+    \<open>\<forall>M. \<nabla>M \<longrightarrow>
+      (M \<Turnstile>\<^sub>M (\<phi>\<^sub>1 \<^bold>\<or> \<phi>\<^sub>2) \<and> M \<Turnstile>\<^sub>E (enabledb a) \<longrightarrow> the (\<M> a M) \<Turnstile>\<^sub>M \<psi>) \<and> 
+      (M \<Turnstile>\<^sub>M (\<phi>\<^sub>1 \<^bold>\<or> \<phi>\<^sub>2) \<and> M \<Turnstile>\<^sub>E \<^bold>\<not>(enabledb a) \<longrightarrow> M \<Turnstile>\<^sub>M \<psi>)\<close>
+  proof
+    fix M
+    show \<open>\<nabla>M \<longrightarrow>
+      (M \<Turnstile>\<^sub>M (\<phi>\<^sub>1 \<^bold>\<or> \<phi>\<^sub>2) \<and> M \<Turnstile>\<^sub>E (enabledb a) \<longrightarrow> the (\<M> a M) \<Turnstile>\<^sub>M \<psi>) \<and> 
+      (M \<Turnstile>\<^sub>M (\<phi>\<^sub>1 \<^bold>\<or> \<phi>\<^sub>2) \<and> M \<Turnstile>\<^sub>E \<^bold>\<not>(enabledb a) \<longrightarrow> M \<Turnstile>\<^sub>M \<psi>)\<close>
+    proof
+      assume \<open>\<nabla>M\<close>
+      show 
+        \<open>(M \<Turnstile>\<^sub>M (\<phi>\<^sub>1 \<^bold>\<or> \<phi>\<^sub>2) \<and> M \<Turnstile>\<^sub>E (enabledb a) \<longrightarrow> the (\<M> a M) \<Turnstile>\<^sub>M \<psi>) \<and> 
+         (M \<Turnstile>\<^sub>M (\<phi>\<^sub>1 \<^bold>\<or> \<phi>\<^sub>2) \<and> M \<Turnstile>\<^sub>E \<^bold>\<not>(enabledb a) \<longrightarrow> M \<Turnstile>\<^sub>M \<psi>)\<close> 
+      proof
+        show \<open>M \<Turnstile>\<^sub>M (\<phi>\<^sub>1 \<^bold>\<or> \<phi>\<^sub>2) \<and> M \<Turnstile>\<^sub>E (enabledb a) \<longrightarrow> the (\<M> a M) \<Turnstile>\<^sub>M \<psi>\<close> 
+        proof
+          assume \<open>M \<Turnstile>\<^sub>M (\<phi>\<^sub>1 \<^bold>\<or> \<phi>\<^sub>2) \<and> M \<Turnstile>\<^sub>E (enabledb a)\<close> 
+          moreover from rDis(2) have \<open>M \<Turnstile>\<^sub>M \<phi>\<^sub>1 \<and> M \<Turnstile>\<^sub>E (enabledb a) \<longrightarrow> the (\<M> a M) \<Turnstile>\<^sub>M \<psi>\<close>
+            using \<open>\<nabla>M\<close> transfer_semantics\<^sub>M semantics\<^sub>H.simps(1) semantics\<^sub>P.simps(5) by blast
+          moreover from rDis(4) have \<open>M \<Turnstile>\<^sub>M \<phi>\<^sub>2 \<and> M \<Turnstile>\<^sub>E (enabledb a) \<longrightarrow> the (\<M> a M) \<Turnstile>\<^sub>M \<psi>\<close>
+            using \<open>\<nabla>M\<close> transfer_semantics\<^sub>M semantics\<^sub>H.simps(1) semantics\<^sub>P.simps(5) by blast
+          ultimately show \<open>the (\<M> a M) \<Turnstile>\<^sub>M \<psi>\<close> by auto
+        qed
+        show \<open>M \<Turnstile>\<^sub>M (\<phi>\<^sub>1 \<^bold>\<or> \<phi>\<^sub>2) \<and> M \<Turnstile>\<^sub>E \<^bold>\<not>(enabledb a) \<longrightarrow> M \<Turnstile>\<^sub>M \<psi>\<close>
+        proof
+          assume \<open>M \<Turnstile>\<^sub>M (\<phi>\<^sub>1 \<^bold>\<or> \<phi>\<^sub>2) \<and> M \<Turnstile>\<^sub>E \<^bold>\<not>(enabledb a)\<close> 
+          moreover from rDis(2) have \<open>M \<Turnstile>\<^sub>M \<phi>\<^sub>1 \<and> M \<Turnstile>\<^sub>E \<^bold>\<not>(enabledb a) \<longrightarrow> M \<Turnstile>\<^sub>M \<psi>\<close>
+            using \<open>\<nabla>M\<close> transfer_semantics\<^sub>M semantics\<^sub>H.simps(1) semantics\<^sub>P.simps(5) by blast
+          moreover from rDis(4) have \<open>M \<Turnstile>\<^sub>M \<phi>\<^sub>2 \<and> M \<Turnstile>\<^sub>E \<^bold>\<not>(enabledb a) \<longrightarrow> M \<Turnstile>\<^sub>M \<psi>\<close>
+            using \<open>\<nabla>M\<close> transfer_semantics\<^sub>M semantics\<^sub>H.simps(1) semantics\<^sub>P.simps(5) by blast
+          ultimately show \<open>M \<Turnstile>\<^sub>M \<psi>\<close> by auto
+        qed
+      qed
+    qed
+  qed
+  with transfer_semantics\<^sub>M show ?case by simp
+qed auto
 
+(* Probably won't show this anytime soon... 
 theorem completeness\<^sub>H: \<open>\<Turnstile>\<^sub>H H \<Longrightarrow> \<turnstile>\<^sub>H H\<close>
   sorry
-
+*)
 
 end
-
-section \<open>Example\<close>
-
-\<comment> \<open>To be moved to an example theory file. Proof of concept.\<close>
-
-\<comment> \<open>Set up some notation\<close>
-abbreviation \<open>in_dropzone::\<Phi>\<^sub>L \<equiv> Atom 0\<close>
-abbreviation \<open>in_room::\<Phi>\<^sub>L \<equiv> Atom 1\<close>
-abbreviation \<open>collect_red::\<Phi>\<^sub>L \<equiv> Atom 2\<close>
-abbreviation \<open>goto_dropzone::cap \<equiv> basic 0\<close>
-abbreviation \<open>goto_room::cap \<equiv> basic 1\<close>
-
-\<comment> \<open>Specification of the program\<close>
-abbreviation \<open>\<Pi>\<^sub>x \<equiv> { (B in_dropzone) \<triangleright> do goto_room }\<close>
-abbreviation \<open>M\<^sub>0\<^sub>x \<equiv> ( { in_dropzone }, { collect_red } )\<close>
-abbreviation \<open>S\<^sub>x \<equiv> {(\<top>\<^sub>M, \<^bold>{ B in_dropzone \<^bold>} goto_room \<^bold>{ B in_room \<^bold>})}\<close>
-
-\<comment> \<open>Prove that the example is an instance of the single agent program locale\<close>
-\<comment> \<open>We use a trick where \<T> is simply some function that complies to our definition due Hilbert's epsilon operator i.e. the axiom of choice\<close>
-interpretation example: single_agent_program \<open>SOME \<T>. complies \<Pi>\<^sub>x S\<^sub>x \<T>\<close> \<Pi>\<^sub>x M\<^sub>0\<^sub>x S\<^sub>x
-proof -
-  let ?\<T> = \<open>SOME \<T>. complies \<Pi>\<^sub>x S\<^sub>x \<T>\<close>
-  have \<open>\<exists>x. complies \<Pi>\<^sub>x S\<^sub>x x\<close> unfolding complies_def by auto
-  with someI_ex[where ?P=\<open>complies \<Pi>\<^sub>x S\<^sub>x\<close>] have complies\<^sub>x: \<open>complies \<Pi>\<^sub>x S\<^sub>x ?\<T>\<close> .
-  show \<open>single_agent_program (SOME \<T>. complies \<Pi>\<^sub>x S\<^sub>x \<T>) \<Pi>\<^sub>x M\<^sub>0\<^sub>x S\<^sub>x\<close>
-  proof 
-    show \<open>complies \<Pi>\<^sub>x S\<^sub>x ?\<T>\<close> using complies\<^sub>x .
-  next
-    have \<open>\<nabla> M\<^sub>0\<^sub>x\<close>
-    proof - 
-      have \<open>{in_dropzone} \<not>\<Turnstile>\<^sub>L \<bottom>\<^sub>L\<close> by auto
-      moreover have \<open>in_dropzone \<noteq> collect_red\<close> by simp
-      with neq_atom_not_entail have \<open>{in_dropzone} \<not>\<Turnstile>\<^sub>L collect_red\<close> by metis
-      moreover have \<open>{} \<not>\<Turnstile>\<^sub>L \<^bold>\<not> in_dropzone\<close> by auto
-      ultimately show ?thesis unfolding is_mental_state_def by auto
-    qed
-    then show \<open>\<Pi>\<^sub>x \<noteq> {} \<and> \<nabla> M\<^sub>0\<^sub>x\<close> by simp
-  next
-    from complies\<^sub>x show \<open>\<forall>\<Sigma> a. \<Sigma> \<not>\<Turnstile>\<^sub>L \<bottom>\<^sub>L \<longrightarrow> ?\<T> a \<Sigma> \<noteq> None \<longrightarrow> the (?\<T> a \<Sigma>) \<not>\<Turnstile>\<^sub>L \<bottom>\<^sub>L\<close>
-      unfolding complies_def by simp    
-  next
-    fix a \<Sigma>
-    from complies\<^sub>x show \<open>?\<T> a \<Sigma> \<noteq> None \<longrightarrow> (\<exists>\<phi>. (\<phi>, basic a) \<in> \<Pi>\<^sub>x)\<close> 
-      unfolding complies_def by simp
-  qed
-qed
-
-
 end
