Gvf_Logic.thy
@@ -1,55 +1,75 @@
 (*
-
   Goal verification framework
-    - Logic
-  
-  This theory sets up syntax, semantics and a sequent for classical logic with no quantifiers.
-  The type for atoms is arbitrary to allow reuse in different logic languages to be defined.
-
+  - Logic
 *)
+
+\<comment> \<open>This theory sets up syntax, semantics and a sequent for classical logic with no quantifiers.
+    The type for atoms is arbitrary to allow reuse in different logic languages to be defined.\<close>
+
 theory Gvf_Logic imports "HOL-Library.Multiset" begin
 
 section \<open>Syntax\<close> 
 
-\<comment> \<open>The usual operators in bold are used for a recognizable notation\<close>
+\<comment> \<open>The usual infix operators are in bold to avoid conflict with Isabelle's built-in operators.\<close>
 datatype 'a \<Phi>\<^sub>P = Atom 'a | Negation \<open>'a \<Phi>\<^sub>P\<close> (\<open>\<^bold>\<not>\<close>) | 
                 Implication \<open>'a \<Phi>\<^sub>P\<close> \<open>'a \<Phi>\<^sub>P\<close> (infixr \<open>\<^bold>\<longrightarrow>\<close> 60) | 
                 Disjunction \<open>'a \<Phi>\<^sub>P\<close> \<open>'a \<Phi>\<^sub>P\<close> (infixl \<open>\<^bold>\<or>\<close> 70) | 
                 Conjunction \<open>'a \<Phi>\<^sub>P\<close> \<open>'a \<Phi>\<^sub>P\<close> (infixl \<open>\<^bold>\<and>\<close> 80)
+\<comment> \<open>'a is a type variable for the type of atoms. 
+    An element of this type is parsed to the constructor for Atom.
+    The Boolean operators take one (or two) formula(s) as input (having the same type for atoms).\<close>
 
-\<comment> \<open>Equivalence is defined from existing operators\<close>
+\<comment> \<open>Bi-implication is defined from conjunction and implication.\<close>
 abbreviation Equiv\<^sub>P :: \<open>'a \<Phi>\<^sub>P \<Rightarrow> 'a \<Phi>\<^sub>P \<Rightarrow> 'a \<Phi>\<^sub>P\<close> (infix \<open>\<^bold>\<longleftrightarrow>\<close> 60) where
   \<open>P \<^bold>\<longleftrightarrow> Q \<equiv> P \<^bold>\<longrightarrow> Q \<^bold>\<and> Q \<^bold>\<longrightarrow> P\<close>
 
+\<comment> \<open>Example (untyped free variable atoms).\<close>
+value \<open>Atom P \<^bold>\<longrightarrow> (Atom P \<^bold>\<longrightarrow> Atom Q) \<^bold>\<longrightarrow> Atom Q\<close>
+
 section \<open>Semantics\<close>
 
-\<comment> \<open>The semantics of formulas depend on a given interpretation for atoms\<close>
+\<comment> \<open>The semantics function takes an interpretation and a formula and returns a Boolean.\<close>
 primrec semantics\<^sub>P :: \<open>('a \<Rightarrow> bool) \<Rightarrow> 'a \<Phi>\<^sub>P \<Rightarrow> bool\<close> where
   \<open>semantics\<^sub>P f (Atom x) = f x\<close> |
   \<open>semantics\<^sub>P f (\<^bold>\<not> p) = (\<not>semantics\<^sub>P f p)\<close> |
   \<open>semantics\<^sub>P f (p \<^bold>\<longrightarrow> q) = (semantics\<^sub>P f p \<longrightarrow> semantics\<^sub>P f q)\<close> |
   \<open>semantics\<^sub>P f (p \<^bold>\<or> q) = (semantics\<^sub>P f p \<or> semantics\<^sub>P f q)\<close> |
   \<open>semantics\<^sub>P f (p \<^bold>\<and> q) = (semantics\<^sub>P f p \<and> semantics\<^sub>P f q)\<close>
+\<comment> \<open>The interpretation f is a function from atom (element of type 'a) to Boolean.
+    In the case of an atom the value is looked up and returned.
+    In case of a Boolean operator, we can exploit Isabelle's built-in operators.
+    This could also be achieved by proper coding of if-then structures.\<close>
 
-\<comment> \<open>Entailment is defined\<close>
+\<comment> \<open>Example (holds for any f, P and Q).\<close>
+lemma \<open>semantics\<^sub>P f (Atom P \<^bold>\<longrightarrow> (Atom P \<^bold>\<longrightarrow> Atom Q) \<^bold>\<longrightarrow> Atom Q)\<close> by simp
+
+\<comment> \<open>Entailment.\<close>
 abbreviation entails :: \<open>'a \<Phi>\<^sub>P set \<Rightarrow> 'a \<Phi>\<^sub>P set \<Rightarrow> bool\<close> (infix \<open>\<Turnstile>\<^sub>P#\<close> 50) where
   \<open>\<Gamma> \<Turnstile>\<^sub>P# \<Delta> \<equiv> (\<forall>f. (\<forall>p\<in>\<Gamma>. semantics\<^sub>P f p) \<longrightarrow> (\<exists>p\<in>\<Delta>. semantics\<^sub>P f p))\<close>
+\<comment> \<open>L entails R if, for all interpretations, all formulas in L true implies at least one in R true.\<close>
 
-\<comment> \<open>Entailment for a singleton rhs\<close>
+\<comment> \<open>Example.\<close>
+lemma \<open>{ Atom P } \<Turnstile>\<^sub>P# { Atom P, Atom Q }\<close> by simp
+
+\<comment> \<open>Entailment for a singleton on rhs.\<close>
 abbreviation entails_singleton :: \<open>'a \<Phi>\<^sub>P set \<Rightarrow> 'a \<Phi>\<^sub>P \<Rightarrow> bool\<close> (infix \<open>\<Turnstile>\<^sub>P\<close> 50) where
   \<open>\<Gamma> \<Turnstile>\<^sub>P \<Phi> \<equiv> \<Gamma> \<Turnstile>\<^sub>P# { \<Phi> }\<close>
 
-\<comment> \<open>Not entailed, for a singleton rhs\<close>
-abbreviation not_entails :: \<open>'a \<Phi>\<^sub>P set \<Rightarrow> 'a \<Phi>\<^sub>P \<Rightarrow> bool\<close> (infix \<open>\<not>\<Turnstile>\<^sub>P\<close> 50) where
-  \<open>\<Gamma> \<not>\<Turnstile>\<^sub>P \<Phi> \<equiv> \<not>(\<forall>f. (\<forall>p\<in>\<Gamma>. semantics\<^sub>P f p) \<longrightarrow> semantics\<^sub>P f \<Phi>)\<close>
+\<comment> \<open>Example.\<close>
+lemma \<open>{ Atom P \<^bold>\<and> Atom Q } \<Turnstile>\<^sub>P Atom P\<close> by simp
+
+\<comment> \<open>Example.\<close>
+lemma \<open>Q \<noteq> P \<longrightarrow> \<not> { Atom Q } \<Turnstile>\<^sub>P Atom P\<close> by auto
 
 \<comment> \<open>Weakening of assumptions for entailment\<close>
-lemma weakening_entailment: \<open>\<Sigma>' \<subseteq> \<Sigma> \<longrightarrow> \<Sigma>' \<Turnstile>\<^sub>P# \<Gamma> \<longrightarrow> \<Sigma> \<Turnstile>\<^sub>P# \<Gamma>\<close>
-  by blast
+lemma weakening_entailment: \<open>\<Sigma>' \<subseteq> \<Sigma> \<longrightarrow> \<Sigma>' \<Turnstile>\<^sub>P# \<Gamma> \<longrightarrow> \<Sigma> \<Turnstile>\<^sub>P# \<Gamma>\<close>  by blast
+
+\<comment> \<open>Example.\<close>
+lemma \<open>{ P\<^sub>1, P\<^sub>2 } \<Turnstile>\<^sub>P# { Q } \<longrightarrow> { P\<^sub>1, P\<^sub>2, P\<^sub>3 } \<Turnstile>\<^sub>P# { Q }\<close> using weakening_entailment by simp
 
 section \<open>Sequent calculus\<close>
 
-\<comment> \<open>A standard sequent calculus proof system\<close>
+\<comment> \<open>A standard sequent calculus proof system.\<close>
 inductive sequent_calculus :: \<open>'a \<Phi>\<^sub>P multiset \<Rightarrow> 'a \<Phi>\<^sub>P multiset \<Rightarrow> bool\<close> (infix \<open>\<turnstile>\<^sub>P#\<close> 40) where
   \<comment> \<open>Non-branching\<close>
   Axiom:  \<open>{# p #} + \<Gamma> \<turnstile>\<^sub>P# \<Delta> + {# p #}\<close> |
@@ -62,22 +82,50 @@ inductive sequent_calculus :: \<open>'a \<Phi>\<^sub>P multiset \<Rightarrow> 'a
   R_And:  \<open>\<Gamma> \<turnstile>\<^sub>P# \<Delta> + {# p #} \<Longrightarrow> \<Gamma> \<turnstile>\<^sub>P# \<Delta> + {# q #} \<Longrightarrow> \<Gamma> \<turnstile>\<^sub>P# \<Delta> + {# p \<^bold>\<and> q #}\<close> |
   L_Or:   \<open>\<Gamma> + {# p #} \<turnstile>\<^sub>P# \<Delta> \<Longrightarrow> \<Gamma> + {# q #} \<turnstile>\<^sub>P# \<Delta> \<Longrightarrow> \<Gamma> + {# p \<^bold>\<or> q #} \<turnstile>\<^sub>P# \<Delta>\<close> |
   L_Imp:  \<open>\<Gamma> \<turnstile>\<^sub>P# \<Delta> + {# p #} \<Longrightarrow> \<Gamma> + {# q #} \<turnstile>\<^sub>P# \<Delta> \<Longrightarrow> \<Gamma> + {# p \<^bold>\<longrightarrow> q #} \<turnstile>\<^sub>P# \<Delta>\<close>
+\<comment> \<open>The arrow ==> signifies that the rightmost predicate (must be of the inductive type) may be
+    introduced following proof of the assumptions. Axioms may either be directly introduced,
+    or follow from non-inductive preconditions. The inductive rules specify the construction of
+    more complex proofs from existing ones.\<close>
 
-\<comment> \<open>Notation for empty lhs and singleton rhs\<close>
+\<comment> \<open>Example.\<close>
+lemma \<open>{# Atom P \<^bold>\<and> Atom Q #} \<turnstile>\<^sub>P# {# Atom P #}\<close> using L_And Axiom by fastforce
+
+\<comment> \<open>Notation for empty lhs and singleton rhs.\<close>
 abbreviation provable :: \<open>'a \<Phi>\<^sub>P \<Rightarrow> bool\<close> (\<open>\<turnstile>\<^sub>P _\<close> 40) where
   \<open>\<turnstile>\<^sub>P p \<equiv> {#} \<turnstile>\<^sub>P# {# p #}\<close>
 
+\<comment> \<open>Example single-step.\<close>
+lemma \<open>\<turnstile>\<^sub>P Atom P \<^bold>\<longrightarrow> (Atom P \<^bold>\<longrightarrow> Atom Q) \<^bold>\<longrightarrow> Atom Q\<close> 
+proof -
+  from R_Imp have \<open>{#} \<turnstile>\<^sub>P# {# Atom P \<^bold>\<longrightarrow> (Atom P \<^bold>\<longrightarrow> Atom Q) \<^bold>\<longrightarrow> Atom Q #}\<close>
+    if \<open>{# Atom P #} \<turnstile>\<^sub>P# {# (Atom P \<^bold>\<longrightarrow> Atom Q) \<^bold>\<longrightarrow> Atom Q #}\<close> using that by simp
+  with R_Imp have ?thesis 
+    if \<open>{# Atom P \<^bold>\<longrightarrow> Atom Q, Atom P #} \<turnstile>\<^sub>P# {# Atom Q #}\<close> using that by auto
+  with L_Imp have ?thesis 
+    if  \<open>{# Atom P #} \<turnstile>\<^sub>P# {# Atom Q #} + {# Atom P #}\<close>
+    and \<open>{# Atom P #} + {# Atom Q #} \<turnstile>\<^sub>P# {# Atom Q #}\<close> using that by auto
+  with Axiom show ?thesis by auto
+qed
+\<comment> \<open>The hassle of manually proving even simple formulas calls for an implementation of proof tactics.
+    The deep embedding of the logic means that trivial formulas cannot be proved using Isabelle's
+    vast knowledge about logic formulas, however I am not sure if there is a good  way around this.\<close>
+
 section \<open>Soundness\<close>
 
-\<comment> \<open>The soundness theorem requires multiset to set conversion\<close>
+\<comment> \<open>The soundness theorem.\<close>
 theorem soundness\<^sub>P: \<open>\<Gamma> \<turnstile>\<^sub>P# \<Delta> \<Longrightarrow> set_mset \<Gamma> \<Turnstile>\<^sub>P# set_mset \<Delta>\<close>
   by (induct rule: sequent_calculus.induct) (auto)
+\<comment> \<open>Proving the formula implies that it is valid. Because the sequent calculus is based on the use
+    of multisets, whereas the semantics is based on regular sets, a conversion is required.
+    In general going from multisets to sets is more clean due to the former always being finite.\<close>
 
 section \<open>Collection of semantic rules\<close>
 
+\<comment> \<open>Proofs about the formulas that are not entailed are in general harder, so the idea is to collect
+    a number of proofs in a small library as we encounter the need to complete such proofs.\<close>
 lemma neq_atom_not_entail: 
   assumes \<open>x \<noteq> y\<close> 
-  shows   \<open>{ Atom x } \<not>\<Turnstile>\<^sub>P Atom y\<close> 
-using assms by auto
+  shows   \<open>\<not> { Atom x } \<Turnstile>\<^sub>P Atom y\<close> 
+  using assms by auto
 
 end
