Gvf_Mental_States.thy
@@ -1,45 +1,51 @@
 (*
-
   Goal verification framework
     - Mental States
-  
-  This theory introduces mental states and mental state formulas.
-  The syntax and semantics of mental state formulas is defined.
-  A proof system for mental state formulas is proved sound.
-
 *)
+
+\<comment> \<open>This theory introduces mental states and mental state formulas.
+  The syntax and semantics of mental state formulas is defined.
+  A proof system for mental state formulas is proved sound.\<close>
+
 theory Gvf_Mental_States imports Gvf_PL begin
                                       
 section \<open>Properties of mental states\<close>
 
-\<comment> \<open>We set up a type for mental states\<close>
-type_synonym mental_state = \<open>(\<Phi>\<^sub>L set \<times> \<Phi>\<^sub>L set)\<close> 
+\<comment> \<open>We set up a type for mental states.\<close>
+type_synonym mental_state = \<open>(\<Phi>\<^sub>L set \<times> \<Phi>\<^sub>L set)\<close>
+\<comment> \<open>A mental state is a tuple of sets of propositional logic formulas.\<close>
 
-\<comment> \<open>The definition constrains elements of the type and may be introduced where needed.\<close>
+\<comment> \<open>The definition filters those elements that are 'tuples of sets of propositional logic formulas'.
+    Not all elements of this type are in fact mental states: a number of restrictions apply.\<close>
 definition is_mental_state :: \<open>mental_state \<Rightarrow> bool\<close> (\<open>\<nabla>\<close>) where
-  \<open>\<nabla> x \<equiv> let (\<Sigma>, \<Gamma>) = x in 
-    \<Sigma> \<not>\<Turnstile>\<^sub>L \<bottom>\<^sub>L           \<comment> \<open>\<Sigma> is consistent\<close>
-      \<and> (\<forall>\<gamma>\<in>\<Gamma>.                    \<comment> \<open>for any \<gamma> \<in> \<Gamma>\<close>
-        \<Sigma> \<not>\<Turnstile>\<^sub>L \<gamma>              \<comment> \<open>(i) \<gamma> is not entailed by the agent's beliefs\<close> 
-        \<and> {} \<not>\<Turnstile>\<^sub>L \<^bold>\<not> \<gamma>)\<close>   \<comment> \<open>(ii) \<gamma> is consistent\<close>
+  \<open>\<nabla> M \<equiv> let (\<Sigma>, \<Gamma>) = M in \<comment> \<open>Pattern matching to have variables for belief and goal base.\<close> 
+    \<not> \<Sigma> \<Turnstile>\<^sub>L \<bottom>\<^sub>L \<comment> \<open>\<Sigma> is consistent.\<close>
+      \<and> (\<forall>\<gamma>\<in>\<Gamma>. \<comment> \<open>for all goals \<gamma> \<in> \<Gamma>:\<close>
+        \<not> \<Sigma> \<Turnstile>\<^sub>L \<gamma> \<comment> \<open>(i) \<gamma> is not entailed by the agent's beliefs,\<close> 
+        \<and> \<not> {} \<Turnstile>\<^sub>L \<^bold>\<not> \<gamma>)\<close> \<comment> \<open>(ii) \<gamma> is consistent.\<close>
+\<comment> \<open>Note that the subgoal property for goals is missing. It will be defined in the semantics.\<close>
 
-\<comment> \<open>If \<gamma>' is weaker than a consistent formula \<gamma>, it must itself be consistent\<close>
+\<comment> \<open>If \<gamma>' is weaker than a consistent formula \<gamma>, it must itself be consistent.\<close>
 lemma \<open>\<not> {} \<Turnstile>\<^sub>L \<^bold>\<not> \<gamma> \<longrightarrow> {} \<Turnstile>\<^sub>L \<gamma> \<^bold>\<longrightarrow> \<gamma>' \<longrightarrow> \<not> {} \<Turnstile>\<^sub>L \<^bold>\<not> \<gamma>'\<close>
   by force
 
-\<comment> \<open>Every member (of the goal set) must be weaker than \<bottom>, but not weaker than any belief \<sigma>\<close>
+\<comment> \<open>Every member (of the goal set) must be weaker than \<bottom>, but not weaker than any belief \<sigma>.\<close>
 lemma \<open>\<nabla> (\<Sigma>, \<Gamma>) \<longrightarrow> (\<forall>\<gamma>\<in>\<Gamma>. {} \<Turnstile>\<^sub>L \<bottom>\<^sub>L \<^bold>\<longrightarrow> \<gamma> \<and> \<not> (\<exists>\<sigma>\<in>\<Sigma>. {} \<Turnstile>\<^sub>L \<sigma> \<^bold>\<longrightarrow> \<gamma>))\<close>
   unfolding is_mental_state_def by fastforce
 
 section \<open>Syntax of mental state formulas\<close>
 
-\<comment> \<open>Atoms are now the special belief and goal modalities\<close>
+\<comment> \<open>Atoms are now the special belief and goal modalities.\<close>
 datatype Atoms\<^sub>M = Bl \<Phi>\<^sub>L | Gl \<Phi>\<^sub>L
+\<comment> \<open>We now use a more complex type for atoms compared to simply natural numbers.
+    Bl and Gl are the constructors taking a propositional logic formula as input.
+    We will introduce a nicer syntax below that hides the nested constructors.\<close>
 
-\<comment> \<open>We set up a type for mental state formulas\<close>
+\<comment> \<open>We set up a type for mental state formulas.\<close>
 type_synonym \<Phi>\<^sub>M = \<open>Atoms\<^sub>M \<Phi>\<^sub>P\<close>
+\<comment> \<open>We instantiate the general logic parsing the type for atoms.\<close>
 
-\<comment> \<open>We hide the nesting in the notation\<close>
+\<comment> \<open>We introduce syntax translations that hide the nesting in the notation.\<close>
 syntax
   "_G" :: \<open>\<Phi>\<^sub>L \<Rightarrow> \<Phi>\<^sub>M\<close>  (\<open>G _\<close> 55)
   "_B" :: \<open>\<Phi>\<^sub>L \<Rightarrow> \<Phi>\<^sub>M\<close>  (\<open>B _\<close> 55)
@@ -47,6 +53,7 @@ translations
   "G \<Phi>" \<rightharpoonup> "(Gvf_Logic.Atom (Atoms\<^sub>M.Gl \<Phi>))"
   "B \<Phi>" \<rightharpoonup> "(Gvf_Logic.Atom (Atoms\<^sub>M.Bl \<Phi>))"
 
+\<comment> \<open>Again truth and falsity are defined for this instance of the logic from a simple tautology.\<close>
 abbreviation Truth\<^sub>M :: \<open>\<Phi>\<^sub>M\<close> (\<open>\<top>\<^sub>M\<close>) where 
   \<open>\<top>\<^sub>M \<equiv> \<^bold>\<not> (B (Atom 0)) \<^bold>\<or> (B (Atom 0))\<close>
 abbreviation Falsity\<^sub>L :: \<open>\<Phi>\<^sub>M\<close> (\<open>\<bottom>\<^sub>M\<close>) where 
@@ -54,27 +61,54 @@ abbreviation Falsity\<^sub>L :: \<open>\<Phi>\<^sub>M\<close> (\<open>\<bottom>\
 
 section \<open>Semantics\<close>
 
-\<comment> \<open>Semantics of atoms for mental state formulas is derived given a mental state\<close>
-primrec semantics\<^sub>M' :: \<open>mental_state \<Rightarrow> Atoms\<^sub>M \<Rightarrow> bool\<close> where
-  \<open>semantics\<^sub>M' M (Bl \<Phi>) = (let (\<Sigma>, _) = M in \<Sigma> \<Turnstile>\<^sub>L \<Phi>)\<close> |
-  \<comment> \<open>The subgoal property for goals is defined in the semantics to avoid problems\<close>
-  \<open>semantics\<^sub>M' M (Gl \<Phi>) = (let (\<Sigma>, \<Gamma>) = M in \<Sigma> \<not>\<Turnstile>\<^sub>L \<Phi> \<and> (\<exists>\<gamma>\<in>\<Gamma>. {} \<Turnstile>\<^sub>L \<gamma> \<^bold>\<longrightarrow> \<Phi>))\<close>
+\<comment> \<open>Semantics of atoms for mental state formulas is derived given a mental state.\<close>
+fun semantics\<^sub>M' :: \<open>mental_state \<Rightarrow> Atoms\<^sub>M \<Rightarrow> bool\<close> where
+\<comment> \<open>Does the belief base entail \<Phi>?\<close>
+  \<open>semantics\<^sub>M' (\<Sigma>, _) (Bl \<Phi>) = (\<Sigma> \<Turnstile>\<^sub>L \<Phi>)\<close> |
+\<comment> \<open>Is \<Phi> not entailed by the belief base and a (sub)goal?\<close>
+  \<open>semantics\<^sub>M' (\<Sigma>, \<Gamma>) (Gl \<Phi>) = (\<not> \<Sigma> \<Turnstile>\<^sub>L \<Phi> \<and> (\<exists>\<gamma>\<in>\<Gamma>. {} \<Turnstile>\<^sub>L \<gamma> \<^bold>\<longrightarrow> \<Phi>))\<close>
 
-\<comment> \<open>We reuse the semantics of the usual logical operators\<close>
+\<comment> \<open>Semantics of formulas.\<close>
 abbreviation semantics\<^sub>M :: \<open>mental_state \<Rightarrow> \<Phi>\<^sub>M \<Rightarrow> bool\<close> (infix \<open>\<Turnstile>\<^sub>M\<close> 50) where
   \<open>M \<Turnstile>\<^sub>M \<phi> \<equiv> semantics\<^sub>P (semantics\<^sub>M' M) \<phi>\<close>
+\<comment> \<open>The semantics for atoms, given a mental state, matches the type for an interpretation.
+    The curried function is parsed on to the general semantics as an interpretation which allows
+    reuse of the existing definition.\<close>
+
+\<comment> \<open>Examples.\<close>
+lemma \<open>({ \<Phi> }, {}) \<Turnstile>\<^sub>M B \<Phi>\<close> by simp
+
+lemma \<open>({ Atom 0 }, { Atom 2 }) \<Turnstile>\<^sub>M G (Atom 1 \<^bold>\<longrightarrow> Atom 2)\<close> (is \<open>({ ?R }, { ?Q }) \<Turnstile>\<^sub>M G (?P \<^bold>\<longrightarrow> ?Q)\<close>)
+proof -
+  have \<open>?R \<noteq> ?Q\<close> by simp
+  have \<open>\<not> { ?R } \<Turnstile>\<^sub>P ?P \<^bold>\<longrightarrow> ?Q\<close>
+  proof 
+    assume \<open>{ ?R } \<Turnstile>\<^sub>P ?P \<^bold>\<longrightarrow> ?Q\<close>
+    then have \<open>\<forall>f. semantics\<^sub>P f ?R \<longrightarrow> semantics\<^sub>P f (?P \<^bold>\<longrightarrow> ?Q)\<close> by auto
+    moreover have \<open>\<exists>f. \<not> (semantics\<^sub>P f ?R \<longrightarrow> semantics\<^sub>P f (?P \<^bold>\<longrightarrow> ?Q))\<close>
+    proof
+      let ?f = \<open>(\<lambda>_. True)((0::nat) := True, 1 := True, 2 := False)\<close>
+      show \<open>\<not> (semantics\<^sub>P ?f ?R \<longrightarrow> semantics\<^sub>P ?f (?P \<^bold>\<longrightarrow> ?Q))\<close> by simp
+    qed
+    ultimately show False by auto
+  qed
+  then have \<open>\<not> { Atom 0 } \<Turnstile>\<^sub>L (Atom 1 \<^bold>\<longrightarrow> Atom 2)\<close> by simp
+  moreover have \<open>{} \<Turnstile>\<^sub>L Atom 2 \<^bold>\<longrightarrow> (Atom 1 \<^bold>\<longrightarrow> Atom 2)\<close> by simp
+  then have \<open>\<exists>\<gamma>\<in>{ Atom 2 }. {} \<Turnstile>\<^sub>L \<gamma> \<^bold>\<longrightarrow> (Atom 1 \<^bold>\<longrightarrow> Atom 2)\<close> by simp
+  ultimately show ?thesis by simp
+qed
 
 section \<open>Various proofs\<close>
 
-\<comment> \<open>An agent cannot have a goal to achieve a tautology\<close>
+\<comment> \<open>An agent cannot have a goal to achieve a tautology.\<close>
 lemma \<open>\<nabla> M \<longrightarrow> \<not> M \<Turnstile>\<^sub>M G \<top>\<^sub>L\<close> 
   unfolding is_mental_state_def by auto
 
-\<comment> \<open>An agent does not have inconsistent beliefs/goals\<close>
+\<comment> \<open>An agent does not have inconsistent beliefs/goals.\<close>
 lemma not_modal_False: \<open>\<nabla> M \<longrightarrow> M \<Turnstile>\<^sub>M \<^bold>\<not> (B \<bottom>\<^sub>L)\<close> \<open>\<nabla> M \<longrightarrow> M \<Turnstile>\<^sub>M \<^bold>\<not> (G \<bottom>\<^sub>L)\<close>
-  unfolding is_mental_state_def by auto
+  unfolding is_mental_state_def by fastforce+
 
-\<comment> \<open>Properties of the goal modality\<close>
+\<comment> \<open>Properties of the goal modality.\<close>
 lemma G_properties:
   shows \<open>\<not> (\<forall>\<Sigma> \<Gamma> \<Phi> \<psi>. \<nabla> (\<Sigma>, \<Gamma>) \<longrightarrow> (\<Sigma>, \<Gamma>) \<Turnstile>\<^sub>M (G \<Phi> \<^bold>\<longrightarrow> \<psi>) \<^bold>\<longrightarrow> (G \<Phi>) \<^bold>\<longrightarrow> (G \<psi>))\<close>
     and \<open>\<not> (\<forall>\<Sigma> \<Gamma> \<Phi> \<psi>. \<nabla> (\<Sigma>, \<Gamma>) \<longrightarrow> (\<Sigma>, \<Gamma>) \<Turnstile>\<^sub>M (G \<Phi> \<^bold>\<and> (\<Phi> \<^bold>\<longrightarrow> \<psi>)) \<^bold>\<longrightarrow> (G \<psi>))\<close>
@@ -86,7 +120,7 @@ proof -
   show \<open>\<not> (\<forall>\<Sigma> \<Gamma> \<Phi> \<psi>. \<nabla> (\<Sigma>, \<Gamma>) \<longrightarrow> (\<Sigma>, \<Gamma>) \<Turnstile>\<^sub>M (G (\<Phi> \<^bold>\<longrightarrow> \<psi>)) \<^bold>\<longrightarrow> (G \<Phi>) \<^bold>\<longrightarrow> (G \<psi>))\<close>
   proof 
     assume *: \<open>\<forall>\<Sigma> \<Gamma> \<Phi> \<psi>. \<nabla> (\<Sigma>, \<Gamma>) \<longrightarrow> (\<Sigma>, \<Gamma>) \<Turnstile>\<^sub>M (G \<Phi> \<^bold>\<longrightarrow> \<psi>) \<^bold>\<longrightarrow> (G \<Phi>) \<^bold>\<longrightarrow> (G \<psi>)\<close>
-    \<comment> \<open>Counter example\<close>
+    \<comment> \<open>Counter example.\<close>
     let ?\<Sigma> = \<open>{}\<close> and ?\<Gamma> = \<open>{ ?\<Phi> \<^bold>\<longrightarrow> ?\<psi>, ?\<Phi> }\<close>
     have \<open>\<not> (?\<Sigma>, ?\<Gamma>) \<Turnstile>\<^sub>M (G ?\<Phi> \<^bold>\<longrightarrow> ?\<psi>) \<^bold>\<longrightarrow> (G ?\<Phi>) \<^bold>\<longrightarrow> (G ?\<psi>)\<close> by auto
     moreover have \<open>\<nabla> (?\<Sigma>, ?\<Gamma>)\<close> unfolding is_mental_state_def by auto
@@ -95,7 +129,7 @@ proof -
   show \<open>\<not> (\<forall>\<Sigma> \<Gamma> \<Phi> \<psi>. \<nabla> (\<Sigma>, \<Gamma>) \<longrightarrow> (\<Sigma>, \<Gamma>) \<Turnstile>\<^sub>M (G \<Phi> \<^bold>\<and> (\<Phi> \<^bold>\<longrightarrow> \<psi>)) \<^bold>\<longrightarrow> (G \<psi>))\<close>
   proof
     assume *: \<open>\<forall>\<Sigma> \<Gamma> \<Phi> \<psi>. \<nabla> (\<Sigma>, \<Gamma>) \<longrightarrow> (\<Sigma>, \<Gamma>) \<Turnstile>\<^sub>M (G \<Phi> \<^bold>\<and> (\<Phi> \<^bold>\<longrightarrow> \<psi>)) \<^bold>\<longrightarrow> (G \<psi>)\<close>
-    \<comment> \<open>Counter example\<close>
+    \<comment> \<open>Counter example.\<close>
     let ?\<Sigma> = \<open>{ ?\<psi> }\<close> and ?\<Gamma> = \<open>{ ?\<Phi> \<^bold>\<and> (?\<Phi> \<^bold>\<longrightarrow> ?\<psi>) }\<close>
     have \<open>\<not> (?\<Sigma>, ?\<Gamma>) \<Turnstile>\<^sub>M (G ?\<Phi> \<^bold>\<and> (?\<Phi> \<^bold>\<longrightarrow> ?\<psi>)) \<^bold>\<longrightarrow> (G ?\<psi>)\<close>
       by auto
@@ -105,7 +139,7 @@ proof -
   show \<open>\<not> (\<forall>\<Sigma> \<Gamma> \<Phi> \<psi>. \<nabla> (\<Sigma>, \<Gamma>) \<longrightarrow> (\<Sigma>, \<Gamma>) \<Turnstile>\<^sub>M (G \<Phi>) \<^bold>\<and> (G \<psi>) \<^bold>\<longrightarrow> (G \<Phi> \<^bold>\<and> \<psi>))\<close>
   proof
     assume *: \<open>\<forall>\<Sigma> \<Gamma> \<Phi> \<psi>. \<nabla> (\<Sigma>, \<Gamma>) \<longrightarrow> (\<Sigma>, \<Gamma>) \<Turnstile>\<^sub>M (G \<Phi>) \<^bold>\<and> (G \<psi>) \<^bold>\<longrightarrow> (G \<Phi> \<^bold>\<and> \<psi>)\<close>
-    \<comment> \<open>Counter example\<close>
+    \<comment> \<open>Counter example.\<close>
     let ?\<Sigma> = \<open>{}\<close> and 
         ?\<Gamma> = \<open>{ ?\<Phi>, ?\<psi> }\<close>
     have \<open>\<not> (?\<Sigma>, ?\<Gamma>) \<Turnstile>\<^sub>M (G ?\<Phi>) \<^bold>\<and> (G ?\<psi>) \<^bold>\<longrightarrow> (G ?\<Phi> \<^bold>\<and> ?\<psi>)\<close>
@@ -121,22 +155,35 @@ qed
 
 section \<open>Provability\<close>
 
-\<comment> \<open>A proof system for mental state formulas\<close>
+\<comment> \<open>A proof system for mental state formulas.\<close>
 inductive derive\<^sub>M :: \<open>\<Phi>\<^sub>M \<Rightarrow> bool\<close> (\<open>\<turnstile>\<^sub>M _\<close> 40) where
-  \<comment> \<open>Derive classical tautologies\<close>
+  \<comment> \<open>Derive classical tautologies.\<close>
   R1: \<open>\<turnstile>\<^sub>P \<phi> \<Longrightarrow> \<turnstile>\<^sub>M \<phi>\<close> |
-  \<comment> \<open>Properties of beliefs\<close> 
+  \<comment> \<open>Properties of beliefs.\<close> 
   R2: \<open>\<turnstile>\<^sub>P \<Phi> \<Longrightarrow> \<turnstile>\<^sub>M (B \<Phi>)\<close> |
   A1: \<open>\<turnstile>\<^sub>M ((B \<Phi> \<^bold>\<longrightarrow> \<psi>) \<^bold>\<longrightarrow> (B \<Phi>) \<^bold>\<longrightarrow> (B \<psi>))\<close> |
   A2: \<open>\<turnstile>\<^sub>M (\<^bold>\<not> (B \<bottom>\<^sub>L))\<close> |
-  \<comment> \<open>Properties of goals\<close>
+  \<comment> \<open>Properties of goals.\<close>
   A3: \<open>\<turnstile>\<^sub>M (\<^bold>\<not> (G \<bottom>\<^sub>L))\<close> |
   A4: \<open>\<turnstile>\<^sub>M ((B \<Phi>) \<^bold>\<longrightarrow> (\<^bold>\<not> (G \<Phi>)))\<close> |
   A5: \<open>\<turnstile>\<^sub>P (\<Phi> \<^bold>\<longrightarrow> \<psi>) \<Longrightarrow> \<turnstile>\<^sub>M ((\<^bold>\<not> (B \<psi>)) \<^bold>\<longrightarrow> (G \<Phi>) \<^bold>\<longrightarrow> (G \<psi>))\<close>
+\<comment> \<open>The original definition uses semantic arguments in e.g. A5. Since we have soundness, but
+    not completeness (yet), it may be an idea to switch back. Initially I preferred to keep
+    semantics arguments out of the proof system.\<close>
 
-section\<open>Soundness\<close>
+\<comment> \<open>Example.\<close>
+lemma \<open>\<turnstile>\<^sub>M (B \<Phi>) \<^bold>\<or> (\<^bold>\<not> (B \<Phi>))\<close> (is \<open>\<turnstile>\<^sub>M ?P \<^bold>\<or> \<^bold>\<not> ?P\<close>) 
+proof
+  from R_Or have \<open>\<turnstile>\<^sub>P ?P \<^bold>\<or> \<^bold>\<not> ?P\<close> if \<open>{#} \<turnstile>\<^sub>P# {#} + {# ?P, \<^bold>\<not> ?P #}\<close> using that by auto
+  with R_Neg have \<open>\<turnstile>\<^sub>P ?P \<^bold>\<or> \<^bold>\<not> ?P\<close> if \<open>{# ?P #} \<turnstile>\<^sub>P# {# ?P #}\<close> using that
+    by (metis add_mset_add_single empty_neutral(1) union_commute)
+    (* Multiset is giving some problems with single stepping it seems... *)
+  with Axiom show \<open>\<turnstile>\<^sub>P ?P \<^bold>\<or> \<^bold>\<not> ?P\<close> by auto
+qed
 
-\<comment> \<open>For the soundness theorem we assume the mental state properties for M\<close>
+section \<open>Soundness\<close>
+
+\<comment> \<open>For the soundness theorem we assume the mental state properties for M.\<close>
 theorem soundness\<^sub>M: 
   assumes \<open>\<nabla> M\<close> 
   shows \<open>\<turnstile>\<^sub>M \<Phi> \<Longrightarrow> M \<Turnstile>\<^sub>M \<Phi>\<close>
@@ -145,10 +192,10 @@ proof (induct rule: derive\<^sub>M.induct)
   with soundness\<^sub>P show ?case by fastforce
 next
   case (R2 \<Phi>)
-  with soundness\<^sub>P show ?case by fastforce
+  with soundness\<^sub>P show ?case by (cases M) fastforce
 next
   case (A1 \<Phi> \<psi>)
-  then show ?case by auto
+  then show ?case by (cases M) auto
 next
   case A2
   from not_modal_False(1) show ?case
@@ -171,22 +218,22 @@ next
       have \<open>(\<Sigma>, \<Gamma>) \<Turnstile>\<^sub>M \<^bold>\<not> (B \<psi>) \<longrightarrow> (\<Sigma>, \<Gamma>) \<Turnstile>\<^sub>M (G \<Phi>) \<longrightarrow> (\<Sigma>, \<Gamma>) \<Turnstile>\<^sub>M G \<psi>\<close>
       proof
         assume \<open>(\<Sigma>, \<Gamma>) \<Turnstile>\<^sub>M \<^bold>\<not> (B \<psi>)\<close>
-        then have \<open>\<Sigma> \<not>\<Turnstile>\<^sub>L \<psi>\<close> by simp
+        then have \<open>\<not>\<Sigma> \<Turnstile>\<^sub>L \<psi>\<close> by simp
         show \<open>(\<Sigma>, \<Gamma>) \<Turnstile>\<^sub>M (G \<Phi>) \<longrightarrow> (\<Sigma>, \<Gamma>) \<Turnstile>\<^sub>M G \<psi>\<close>
         proof
           assume \<open>(\<Sigma>, \<Gamma>) \<Turnstile>\<^sub>M G \<Phi>\<close>
-          then have \<open>\<Phi>\<in>\<Gamma> \<or> \<Sigma> \<not>\<Turnstile>\<^sub>L \<Phi> \<and> (\<exists>\<gamma>\<in>\<Gamma>. {} \<Turnstile>\<^sub>L \<gamma> \<^bold>\<longrightarrow> \<Phi>)\<close> by simp
+          then have \<open>\<Phi>\<in>\<Gamma> \<or> \<not>\<Sigma> \<Turnstile>\<^sub>L \<Phi> \<and> (\<exists>\<gamma>\<in>\<Gamma>. {} \<Turnstile>\<^sub>L \<gamma> \<^bold>\<longrightarrow> \<Phi>)\<close> by simp
           then show \<open>(\<Sigma>, \<Gamma>) \<Turnstile>\<^sub>M G \<psi>\<close> 
           proof
             assume \<open>\<Phi> \<in> \<Gamma>\<close>
             with \<open>{} \<Turnstile>\<^sub>L \<Phi> \<^bold>\<longrightarrow> \<psi>\<close> have \<open>(\<exists>\<gamma>\<in>\<Gamma>. {} \<Turnstile>\<^sub>L \<gamma> \<^bold>\<longrightarrow> \<psi>)\<close> by auto
-            with \<open>\<Sigma> \<not>\<Turnstile>\<^sub>L \<psi>\<close> show ?thesis by simp
+            with \<open>\<not>\<Sigma> \<Turnstile>\<^sub>L \<psi>\<close> show ?thesis by simp
           next
-            assume \<open>\<Sigma> \<not>\<Turnstile>\<^sub>L \<Phi> \<and> (\<exists>\<gamma>\<in>\<Gamma>. {} \<Turnstile>\<^sub>L \<gamma> \<^bold>\<longrightarrow> \<Phi>)\<close>
-            then have \<open>\<Sigma> \<not>\<Turnstile>\<^sub>L \<Phi>\<close> \<open>(\<exists>\<gamma>\<in>\<Gamma>. {} \<Turnstile>\<^sub>L \<gamma> \<^bold>\<longrightarrow> \<Phi>)\<close> by simp+
+            assume \<open>\<not> \<Sigma> \<Turnstile>\<^sub>L \<Phi> \<and> (\<exists>\<gamma>\<in>\<Gamma>. {} \<Turnstile>\<^sub>L \<gamma> \<^bold>\<longrightarrow> \<Phi>)\<close>
+            then have \<open>\<not> \<Sigma> \<Turnstile>\<^sub>L \<Phi>\<close> \<open>(\<exists>\<gamma>\<in>\<Gamma>. {} \<Turnstile>\<^sub>L \<gamma> \<^bold>\<longrightarrow> \<Phi>)\<close> by simp+
             from \<open>(\<exists>\<gamma>\<in>\<Gamma>. {} \<Turnstile>\<^sub>L \<gamma> \<^bold>\<longrightarrow> \<Phi>)\<close> have \<open>(\<exists>\<gamma>\<in>\<Gamma>. {} \<Turnstile>\<^sub>L \<gamma> \<^bold>\<longrightarrow> \<psi>)\<close> 
               using \<open>{} \<Turnstile>\<^sub>L \<Phi> \<^bold>\<longrightarrow> \<psi>\<close> by auto
-            with \<open>\<Sigma> \<not>\<Turnstile>\<^sub>L \<psi>\<close> show ?thesis by simp
+            with \<open>\<not> \<Sigma> \<Turnstile>\<^sub>L \<psi>\<close> show ?thesis by simp
           qed 
         qed
       qed
