Gvf_PL.thy
@@ -1,39 +1,41 @@
 (*
-
   Goal verification framework
     - Propositional Logic
-  
-  This theory is an instance of the general logic for propositions that are natural numbers.
+*)  
+ \<comment> \<open>This theory is an instance of the general classical logic for atoms that are natural numbers.\<close> 
 
-*)
 theory Gvf_PL imports Gvf_Logic begin
 
-\<comment> \<open>Define the type for propositional logic\<close>
+\<comment> \<open>Define the type for propositional logic formulas.\<close>
 type_synonym \<Phi>\<^sub>L = \<open>nat \<Phi>\<^sub>P\<close>
+\<comment> \<open>We parse the type for natural numbers to the general logic type and create a type synonym
+   for this instance.\<close>
 
-\<comment> \<open>Truth and falsity are individually defined requiring a set type for atoms\<close>
+\<comment> \<open>Truth and falsity are defined.\<close>
 abbreviation Truth\<^sub>L :: \<open>\<Phi>\<^sub>L\<close> (\<open>\<top>\<^sub>L\<close>) where 
   \<open>\<top>\<^sub>L \<equiv> \<^bold>\<not> (Atom 0) \<^bold>\<or> (Atom 0)\<close>
 abbreviation Falsity\<^sub>L :: \<open>\<Phi>\<^sub>L\<close> (\<open>\<bottom>\<^sub>L\<close>) where 
   \<open>\<bottom>\<^sub>L \<equiv> \<^bold>\<not> \<top>\<^sub>L\<close>
+\<comment> \<open>Since we base the definition on a simple tautology, we can only define this for one instance
+    of the general classical logic as we need to be able to specify atoms.\<close>
 
 section \<open>Semantics\<close>
 
-\<comment> \<open>The semantics is easily obtained from the general definition\<close>
+\<comment> \<open>The semantics is easily obtained from the definition for general classical logic.\<close>
 abbreviation semantics\<^sub>L :: \<open>(nat \<Rightarrow> bool) \<Rightarrow> \<Phi>\<^sub>L \<Rightarrow> bool\<close> where
   \<open>semantics\<^sub>L f p \<equiv> semantics\<^sub>P f p\<close>
+\<comment> \<open>The semantics of PL is computed the same as for the general case with the interpretation being
+    a function from natural numbers (proposition identifiers) to truth values.\<close>
 
-\<comment> \<open>The soundness result is easily proved from the general case\<close>
+\<comment> \<open>The soundness result is easily proved from the general case.\<close>
 lemma soundness\<^sub>L: \<open>\<turnstile>\<^sub>P p \<Longrightarrow> semantics\<^sub>L f p\<close>
   using soundness\<^sub>P by fastforce
 
-\<comment> \<open>Entailment for propositional logic\<close>
+\<comment> \<open>Entailment for propositional logic.\<close>
 abbreviation entails :: \<open>\<Phi>\<^sub>L set \<Rightarrow> \<Phi>\<^sub>L set \<Rightarrow> bool\<close> (infix \<open>\<Turnstile>\<^sub>L#\<close> 50) where
   \<open>\<Gamma> \<Turnstile>\<^sub>L# \<Delta> \<equiv> \<Gamma> \<Turnstile>\<^sub>P# \<Delta>\<close>
 
-abbreviation not_entails :: \<open>\<Phi>\<^sub>L set \<Rightarrow> \<Phi>\<^sub>L \<Rightarrow> bool\<close> (infix \<open>\<not>\<Turnstile>\<^sub>L\<close> 50) where
-  \<open>\<Gamma> \<not>\<Turnstile>\<^sub>L \<Phi> \<equiv> \<Gamma> \<not>\<Turnstile>\<^sub>P \<Phi>\<close>
-
+\<comment> \<open>Cleaner notation for entailment for of singleton rhs.\<close>
 abbreviation entails_singleton :: \<open>\<Phi>\<^sub>L set \<Rightarrow> \<Phi>\<^sub>L \<Rightarrow> bool\<close> (infix \<open>\<Turnstile>\<^sub>L\<close> 50) where
   \<open>\<Gamma> \<Turnstile>\<^sub>L \<Phi> \<equiv> \<Gamma> \<Turnstile>\<^sub>P \<Phi>\<close>
 
